feat: functions

St/Membership.lean
@@ -7,127 +7,128 @@ axiom St : Type
 /- Membership definition -/
 
 
-axiom mem : St → St → Prop
-axiom eqst : St → St → Prop
-notation:50 a " =st " b => eqst a b
+axiom St.mem : St → St → Prop
+axiom St.eq : St → St → Prop
+infix:50 " =st " => St.eq
 
 
 /- St properties -/
 
 
-axiom set_eq (A B : St) :
-    (∀ x : St, mem x A ↔ mem x B) ↔ A =st B
+axiom St.ext (A B : St) :
+    (∀ x : St, St.mem x A ↔ St.mem x B) ↔ A =st B
 
-axiom set_exists_general_uni (A : St) :
-    ∃ S : St, ∀ x : St, mem x S ↔ ∃ y : St, mem y A ∧ mem x y
+axiom St.exists_general_uni (A : St) :
+    ∃ S : St, ∀ x : St, St.mem x S ↔ ∃ y : St, St.mem y A ∧ St.mem x y
 
-axiom set_exists_pair (a b : St) :
-    ∃ S : St, ∀ x : St, mem x S ↔ ((x =st a) ∨ (x =st b))
+axiom St.exists_pair (a b : St) :
+    ∃ S : St, ∀ x : St, St.mem x S ↔ ((x =st a) ∨ (x =st b))
 
-axiom set_exists_pow (A : St) :
-    ∃ S : St, ∀ x : St, mem x S ↔ ∀ y : St, mem y x → mem y A
+axiom St.exists_pow (A : St) :
+    ∃ S : St, ∀ x : St, St.mem x S ↔ ∀ y : St, St.mem y x → St.mem y A
 
-axiom set_exists_empty :
-    ∃ S : St, ∀ x : St, mem x S ↔ False
+axiom St.exists_empty :
+    ∃ S : St, ∀ x : St, St.mem x S ↔ False
 
 
 /- St definitions -/
 
 
-noncomputable def general_uni (A : St) : St :=
-    Classical.choose (set_exists_general_uni A)
+noncomputable def St.general_uni (A : St) : St :=
+    Classical.choose (St.exists_general_uni A)
 
-noncomputable def pair (a b : St) : St :=
-    Classical.choose (set_exists_pair a b)
+noncomputable def St.pair (a b : St) : St :=
+    Classical.choose (St.exists_pair a b)
 
-noncomputable def empty : St :=
-    Classical.choose set_exists_empty
+noncomputable def St.empty : St :=
+    Classical.choose St.exists_empty
 
-noncomputable def singlet (a : St) : St :=
-    pair a a
+noncomputable def St.singlet (a : St) : St :=
+    St.pair a a
 
-noncomputable def uni (A B : St) : St :=
-    general_uni (pair A B)
+noncomputable def St.uni (A B : St) : St :=
+    St.general_uni (St.pair A B)
 
 
 /- St equivalence -/
 
 
 @[refl]
-theorem eqst_refl (A : St) : A =st A := by
-    apply (set_eq A A).mp
+theorem St.eq_rfl (A : St) : A =st A := by
+    apply (St.ext A A).mp
     intro x
     rfl
 
-theorem eqst_symm {A B : St} : (A =st B) → (B =st A) := by
+theorem St.eq_symm {A B : St} : (A =st B) → (B =st A) := by
    intro hAB
-   replace hAB := (set_eq A B).mpr hAB
-   apply (set_eq B A).mp
+   replace hAB := (St.ext A B).mpr hAB
+   apply (St.ext B A).mp
    intro x
    apply Iff.symm
    exact (hAB x)
 
-theorem eqst_trans {A B C : St} :
+theorem St.eq_trans {A B C : St} :
     (A =st B) → (B =st C) → (A =st C) := by
 
   intro hAB hBC
-  replace hAB := (set_eq A B).mpr hAB
-  replace hBC := (set_eq B C).mpr hBC
-  apply (set_eq A C).mp
+  replace hAB := (St.ext A B).mpr hAB
+  replace hBC := (St.ext B C).mpr hBC
+  apply (St.ext A C).mp
   intro x
   apply (Iff.trans (hAB x) (hBC x))
 
-instance : Trans eqst eqst eqst where
-  trans := eqst_trans
+instance : Trans St.eq St.eq St.eq where
+  trans := St.eq_trans
 
-instance : Equivalence eqst :=
+instance : Equivalence St.eq :=
 ⟨
-  eqst_refl,
-  @eqst_symm,
-  @eqst_trans
+  St.eq_rfl,
+  @St.eq_symm,
+  @St.eq_trans
 ⟩
 
 
 @[simp]
-theorem mem_congr_right {A B x : St} (h : A =st B) :
-  mem x A ↔ mem x B :=
+theorem St.mem_congr_right {A B x : St} (h : A =st B) :
+  St.mem x A ↔ St.mem x B :=
 
 
-  (set_eq A B).mpr h x
+  (St.ext A B).mpr h x
 
 
 /- St theorems -/
 
 
-theorem mem_general_uni (A : St) :
-  ∀ x : St, mem x (general_uni A) ↔ ∃ y : St, mem y A ∧ mem x y :=
+theorem St.mem_general_uni (A : St) :
+  ∀ x : St, St.mem x (St.general_uni A) ↔ ∃ y :
+    St, St.mem y A ∧ St.mem x y :=
 
-  Classical.choose_spec (set_exists_general_uni A)
+  Classical.choose_spec (St.exists_general_uni A)
 
-theorem mem_pair (a b : St) :
-  ∀ x : St, mem x (pair a b) ↔ ((x =st a) ∨ (x =st b)) :=
+theorem St.mem_pair (a b : St) :
+  ∀ x : St, St.mem x (St.pair a b) ↔ ((x =st a) ∨ (x =st b)) :=
 
-  Classical.choose_spec (set_exists_pair a b)
+  Classical.choose_spec (St.exists_pair a b)
 
-theorem mem_empty (x : St) : mem x empty ↔ False :=
+theorem St.mem_empty (x : St) : St.mem x St.empty ↔ False :=
 
-  (Classical.choose_spec set_exists_empty) x
+  (Classical.choose_spec St.exists_empty) x
 
-theorem mem_singlet (a : St) :
-  ∀ x : St, mem x (singlet a) ↔ (x =st a) := by
+theorem St.mem_singlet (a : St) :
+  ∀ x : St, St.mem x (St.singlet a) ↔ (x =st a) := by
 
   intro x
 
-  -- mem x (pair a a) <-> x = a
-  unfold singlet
+  -- St.mem x (St.pair a a) <-> x = a
+  unfold St.singlet
 
-  -- (h: mem x (pair a a) ↔ (x = a ∨ x = a))
-  have h := mem_pair a a x
+  -- (h: St.mem x (St.pair a a) ↔ (x = a ∨ x = a))
+  have h := St.mem_pair a a x
 
   constructor
-  · /- mem x (pair a a) -> x = a -/
+  · /- St.mem x (St.pair a a) -> x = a -/
 
-    -- (hxmempair : mem x (pair a a))
+    -- (hxmempair : St.mem x (St.pair a a))
     intro hxmempair
 
     -- (h: x = a ∨ x = a)
@@ -137,7 +138,7 @@ theorem mem_singlet (a : St) :
     · exact ha
     · exact ha
 
-  · /- x = a -> mem x (pair a a) -/
+  · /- x = a -> St.mem x (St.pair a a) -/
 
     intro ha
 
@@ -145,20 +146,20 @@ theorem mem_singlet (a : St) :
         left
         exact ha
 
-    -- (h: mem x (pair a a))
+    -- (h: St.mem x (St.pair a a))
     replace h := h.mpr haha
     exact h
 
-theorem pair_symm (a b : St) : pair a b =st pair b a := by
-    apply (set_eq (pair a b) (pair b a)).mp
+theorem St.pair_symm (a b : St) : St.pair a b =st St.pair b a := by
+    apply (St.ext (St.pair a b) (St.pair b a)).mp
     intro x
 
     have hmemxpair : ∀ c d : St,
-        mem x (pair c d) → mem x (pair d c) := by
+        St.mem x (St.pair c d) → St.mem x (St.pair d c) := by
 
         intro c d hxmemcd
-        apply (mem_pair d c x).mpr
-        have hxeqcxeqd := (mem_pair c d x).mp hxmemcd
+        apply (St.mem_pair d c x).mpr
+        have hxeqcxeqd := (St.mem_pair c d x).mp hxmemcd
         rcases hxeqcxeqd with hxeqc | hxeqd
         · right
           exact hxeqc
@@ -169,164 +170,164 @@ theorem pair_symm (a b : St) : pair a b =st pair b a := by
     · exact (hmemxpair a b)
     · exact (hmemxpair b a)
 
-theorem mem_uni (A B : St) :
-    ∀ x : St, mem x (uni A B) ↔ mem x A ∨ mem x B := by
+theorem St.mem_uni (A B : St) :
+    ∀ x : St, St.mem x (St.uni A B) ↔ St.mem x A ∨ St.mem x B := by
 
-    -- ∀ x : St, mem x (uni A B) ↔ mem x A ∨ mem x B
-    -- exists (uni A B)
+    -- ∀ x : St, St.mem x (St.uni A B) ↔ St.mem x A ∨ St.mem x B
+    -- exists (St.uni A B)
 
-    -- mem x (uni A B) ↔ mem x A ∨ mem x B
+    -- St.mem x (St.uni A B) ↔ St.mem x A ∨ St.mem x B
     intro x
 
-    -- mem x (general_uni (pair A B)) ↔ mem x A ∨ mem x B
-    unfold uni
+    -- St.mem x (St.general_uni (St.pair A B)) ↔ St.mem x A ∨ St.mem x B
+    unfold St.uni
 
-    -- (h1 : mem x (general_uni (pair A B)) ↔
-    --  ∃ y : St, mem y (pair A B) ∧ mem x y)
+    -- (h1 : St.mem x (St.general_uni (St.pair A B)) ↔
+    --  ∃ y : St, St.mem y (St.pair A B) ∧ St.mem x y)
     --
-    have h1 := mem_general_uni (pair A B) x
+    have h1 := St.mem_general_uni (St.pair A B) x
 
     have h2 :
-        (∃ y : St, mem y (pair A B) ∧ mem x y) ↔
-        mem x A ∨ mem x B := by
+        (∃ y : St, St.mem y (St.pair A B) ∧ St.mem x y) ↔
+        St.mem x A ∨ St.mem x B := by
 
         constructor
-        · /- ∃ y : St, mem y (pair A B) ∧ mem x y ->
-            mem x A ∨ mem x B -/
+        · /- ∃ y : St, St.mem y (St.pair A B) ∧ St.mem x y ->
+            St.mem x A ∨ St.mem x B -/
 
-          -- (h: ∃ y : St, mem y (pair A B) ∧ mem x y )
-          -- mem x A ∨ mem x B
+          -- (h: ∃ y : St, St.mem y (St.pair A B) ∧ St.mem x y )
+          -- St.mem x A ∨ St.mem x B
           intro h
 
-          -- (hy_pair : mem y (pair A B))
-          -- (hxy : mem x y)
+          -- (hy_pair : St.mem y (St.pair A B))
+          -- (hxy : St.mem x y)
           obtain ⟨y, hy_pair, hxy⟩ := h
 
           -- (hyAB : y = A ∨ y = B)
-          have hyAB := (mem_pair A B y).mp hy_pair
+          have hyAB := (St.mem_pair A B y).mp hy_pair
 
           rcases hyAB with hyA | hyB
           · /- y = A -/
             left
-            rw [(mem_congr_right hyA).symm]
+            rw [(St.mem_congr_right hyA).symm]
             exact hxy
           · /- y = B -/
             right
-            rw [(mem_congr_right hyB).symm]
+            rw [(St.mem_congr_right hyB).symm]
             exact hxy
 
-        · /- mem x A ∨ mem x B ->
-            ∃ y : St, mem y (pair A B) ∧ mem x y -/
+        · /- St.mem x A ∨ St.mem x B ->
+            ∃ y : St, St.mem y (St.pair A B) ∧ St.mem x y -/
 
           intro h
 
           have hxmemY_ymempairANDxmemY :
-            ∀ y z : St, mem x y → mem y (pair y z) ∧ mem x y := by
+            ∀ y z : St, St.mem x y → St.mem y (St.pair y z) ∧ St.mem x y := by
 
             intro y z hxy
             constructor
-            · /- mem y (pair y z) -/
+            · /- St.mem y (St.pair y z) -/
               have hyyoryz : (y =st y) ∨ (y =st z) := by
                 left
                 rfl
-              have hy_pair := (mem_pair y z y).mpr hyyoryz
+              have hy_pair := (St.mem_pair y z y).mpr hyyoryz
               exact hy_pair
 
-            · /- mem x y -/
+            · /- St.mem x y -/
               exact hxy
 
           rcases h with hxA | hxB
-          · /- hxA: mem x A -/
+          · /- hxA: St.mem x A -/
             exists A
             have hxmemA_AmempairANDxmemA :=
                 (hxmemY_ymempairANDxmemY A B hxA)
             exact hxmemA_AmempairANDxmemA
 
-          · /- hxB: mem x B -/
+          · /- hxB: St.mem x B -/
             exists B
             have hxmemB_BmempairANDxmemB :=
                 (hxmemY_ymempairANDxmemY B A hxB)
-            rw [mem_congr_right (pair_symm B A)] at hxmemB_BmempairANDxmemB
+            rw [St.mem_congr_right (St.pair_symm B A)] at hxmemB_BmempairANDxmemB
             exact hxmemB_BmempairANDxmemB
 
     exact h1.trans h2
 
 
-theorem set_uni (A B : St) :
-    ∃ U : St, ∀ x : St, mem x U ↔ mem x A ∨ mem x B := by
+theorem St.set_uni (A B : St) :
+    ∃ U : St, ∀ x : St, St.mem x U ↔ St.mem x A ∨ St.mem x B := by
 
-    exists (uni A B)
-    exact mem_uni A B
+    exists (St.uni A B)
+    exact St.mem_uni A B
 
-theorem pair_eq_uni_singet (a b : St) :
-    pair a b =st uni (singlet a) (singlet b) := by
+theorem St.pair_eq_uni_singet (a b : St) :
+    St.pair a b =st St.uni (St.singlet a) (St.singlet b) := by
 
-    apply (set_eq (pair a b) (uni (singlet a) (singlet b))).mp
+    apply (St.ext (St.pair a b) (St.uni (St.singlet a) (St.singlet b))).mp
 
     intro x
-    rw [mem_pair a b x]
-    rw [mem_uni (singlet a) (singlet b) x]
-    rw [mem_singlet a x]
-    rw [mem_singlet b x]
+    rw [St.mem_pair a b x]
+    rw [St.mem_uni (St.singlet a) (St.singlet b) x]
+    rw [St.mem_singlet a x]
+    rw [St.mem_singlet b x]
 
-theorem set_non_empty {A : St} (h : (A =st empty) → False) :
-    ∃ x : St, mem x A := by
+theorem St.set_non_empty {A : St} (h : (A =st St.empty) → False) :
+    ∃ x : St, St.mem x A := by
 
-    -- ∃ x : St, mem x A
-    -- ((∃ x : St, mem x A) -> False) -> False
+    -- ∃ x : St, St.mem x A
+    -- ((∃ x : St, St.mem x A) -> False) -> False
     apply Classical.not_not.mp
 
-    -- (hx : (∃ x : St, mem x A) -> False)
-    -- ((∃ x : St, mem x A) -> False) -> False
+    -- (hx : (∃ x : St, St.mem x A) -> False)
+    -- ((∃ x : St, St.mem x A) -> False) -> False
     -- False
     intro hx
 
     -- False
-    -- A = empty
+    -- A = St.empty
     apply h
 
-    -- A = empty
-    -- (x : St) : mem x A ↔ mem x empty
-    apply (set_eq A empty).mp
+    -- A = St.empty
+    -- (x : St) : St.mem x A ↔ St.mem x St.empty
+    apply (St.ext A St.empty).mp
 
-    -- (x : St) : mem x A ↔ mem x empty
-    -- mem x A ↔ mem x empty
+    -- (x : St) : St.mem x A ↔ St.mem x St.empty
+    -- St.mem x A ↔ St.mem x St.empty
     intro x
 
     constructor
-    · /- mem x A -> mem x empty -/
+    · /- St.mem x A -> St.mem x St.empty -/
 
-      -- mem x A -> mem x empty
-      -- (hA : mem x A)
-      -- mem x empty
+      -- St.mem x A -> St.mem x St.empty
+      -- (hA : St.mem x A)
+      -- St.mem x St.empty
       intro hA
 
       exfalso
       apply hx
       exists x
 
-    · /- mem x empyt -> mem x A -/
+    · /- St.mem x empyt -> St.mem x A -/
       intro hempty
       exfalso
-      apply (mem_empty x).mp
+      apply (St.mem_empty x).mp
       exact hempty
 
-theorem uni_ass (A B C : St) :
-    uni (uni A B) C =st uni A (uni B C) := by
+theorem St.uni_ass (A B C : St) :
+    St.uni (St.uni A B) C =st St.uni A (St.uni B C) := by
 
-    apply (set_eq (uni (uni A B) C) (uni A (uni B C))).mp
+    apply (St.ext (St.uni (St.uni A B) C) (St.uni A (St.uni B C))).mp
     intro x
 
     constructor
-    · /- mem x (uni (uni A B) C) -> mem x (uni A (uni B C)) -/
+    · /- St.mem x (St.uni (St.uni A B) C) -> St.mem x (St.uni A (St.uni B C)) -/
 
       intro h
-      rw [mem_uni] at h
-      rw [mem_uni]
-      rw [mem_uni]
+      rw [St.mem_uni] at h
+      rw [St.mem_uni]
+      rw [St.mem_uni]
       rcases h with hAB | hC
       ·
-        rw [mem_uni] at hAB
+        rw [St.mem_uni] at hAB
 
         rcases hAB with hA | hB
         ·
@@ -341,12 +342,12 @@ theorem uni_ass (A B C : St) :
         right
         exact hC
 
-    · /-  mem x (uni A (uni B C)) -> mem x (uni (uni A B) C) -/
+    · /-  St.mem x (St.uni A (St.uni B C)) -> St.mem x (St.uni (St.uni A B) C) -/
 
       intro h
-      rw [mem_uni] at h
-      rw [mem_uni]
-      rw [mem_uni]
+      rw [St.mem_uni] at h
+      rw [St.mem_uni]
+      rw [St.mem_uni]
 
       rcases h with hA | hBC
       ·
@@ -354,7 +355,7 @@ theorem uni_ass (A B C : St) :
         left
         exact hA
       ·
-        rw [mem_uni] at hBC
+        rw [St.mem_uni] at hBC
 
         rcases hBC with hB | hC
         ·
@@ -366,13 +367,13 @@ theorem uni_ass (A B C : St) :
           exact hC
 
 @[simp]
-theorem uni_comm (A B : St) : uni A B =st uni B A := by
+theorem St.uni_comm (A B : St) : St.uni A B =st St.uni B A := by
 
-    apply (set_eq (uni A B) (uni B A )).mp
+    apply (St.ext (St.uni A B) (St.uni B A )).mp
     intro x
 
-    rw [mem_uni]
-    rw [mem_uni]
+    rw [St.mem_uni]
+    rw [St.mem_uni]
     constructor
     · intro h
       apply Or.symm
@@ -382,15 +383,15 @@ theorem uni_comm (A B : St) : uni A B =st uni B A := by
       exact h
 
 @[simp]
-theorem uni_congr_left {A B C : St} (h : A =st B) :
-  uni A C =st uni B C := by
+theorem St.uni_congr_left {A B C : St} (h : A =st B) :
+  St.uni A C =st St.uni B C := by
 
-  apply (set_eq (uni A C) (uni B C)).mp
+  apply (St.ext (St.uni A C) (St.uni B C)).mp
   intro x
 
-  have hxAeqxB : mem x A ↔ mem x B := mem_congr_right h
+  have hxAeqxB : St.mem x A ↔ St.mem x B := St.mem_congr_right h
 
-  simp only [mem_uni]
+  simp only [St.mem_uni]
 
   constructor
   · intro hxAC
@@ -410,20 +411,20 @@ theorem uni_congr_left {A B C : St} (h : A =st B) :
       exact hC
 
 @[simp]
-theorem uni_congr_right {A B C : St} (h : A =st B) :
-  uni C A =st uni C B :=
+theorem St.uni_congr_right {A B C : St} (h : A =st B) :
+  St.uni C A =st St.uni C B :=
 
   calc
-    uni C A
-        =st uni A C := by apply uni_comm
-    _   =st uni B C := by apply uni_congr_left h
-    _   =st uni C B := by apply uni_comm
+    St.uni C A
+        =st St.uni A C := by apply St.uni_comm
+    _   =st St.uni B C := by apply St.uni_congr_left h
+    _   =st St.uni C B := by apply St.uni_comm
 
 
-theorem uni_self (A : St) : uni A A =st A := by
-    apply (set_eq (uni A A) A).mp
+theorem St.uni_idem (A : St) : St.uni A A =st A := by
+    apply (St.ext (St.uni A A) A).mp
     intro x
-    rw [mem_uni]
+    rw [St.mem_uni]
 
     constructor
     · intro h
@@ -434,47 +435,47 @@ theorem uni_self (A : St) : uni A A =st A := by
       left
       exact h
 
-theorem uni_empty (A : St) : uni A empty =st A := by
-    apply (set_eq (uni A empty) A).mp
+theorem St.uni_empty (A : St) : St.uni A St.empty =st A := by
+    apply (St.ext (St.uni A St.empty) A).mp
     intro x
-    rw [mem_uni]
+    rw [St.mem_uni]
 
     constructor
     · intro h
       rcases h with hA | hempty
       · exact hA
       · exfalso
-        apply (mem_empty x).mp
+        apply (St.mem_empty x).mp
         exact hempty
     · intro h
       left
       exact h
 
 
-/- Inter & diff definitions -/
+/- St.inter & diff definitions -/
 
 
-axiom inter : St → St → St
-axiom mem_inter (A B : St) :
-    ∀ x : St, mem x (inter A B) ↔ mem x A ∧ mem x B
+axiom St.inter : St → St → St
+axiom St.mem_inter (A B : St) :
+    ∀ x : St, St.mem x (St.inter A B) ↔ St.mem x A ∧ St.mem x B
 
-axiom diff : St → St → St
-axiom mem_diff (A B : St) :
-    ∀ x : St, mem x (diff A B) ↔ mem x A ∧ (mem x B → False)
+axiom St.diff : St → St → St
+axiom St.mem_diff (A B : St) :
+    ∀ x : St, St.mem x (diff A B) ↔ St.mem x A ∧ (St.mem x B → False)
 
 
-/- Inter congruence -/
+/- St.inter congruence -/
 
 @[simp]
-theorem inter_congr_right {A B C : St} (h : A =st B) :
-  inter A C =st inter B C := by
+theorem St.inter_congr_right {A B C : St} (h : A =st B) :
+  St.inter A C =st St.inter B C := by
 
-  apply (set_eq (inter A C) (inter B C)).mp
+  apply (St.ext (St.inter A C) (St.inter B C)).mp
   intro x
 
-  have hxAeqxB : mem x A ↔ mem x B := mem_congr_right h
+  have hxAeqxB : St.mem x A ↔ St.mem x B := St.mem_congr_right h
 
-  simp only [mem_inter]
+  simp only [St.mem_inter]
 
   constructor
   · intro hxAC
@@ -492,13 +493,13 @@ theorem inter_congr_right {A B C : St} (h : A =st B) :
     · exact hC
 
 
-/- Inter & diff properties -/
+/- St.inter & diff properties -/
 
 
-theorem inter_empty (A : St) : inter A empty =st empty := by
-    apply (set_eq (inter A empty) empty).mp
+theorem St.inter_empty (A : St) : St.inter A St.empty =st St.empty := by
+    apply (St.ext (St.inter A St.empty) St.empty).mp
     intro x
-    rw [mem_inter]
+    rw [St.mem_inter]
 
     constructor
     · intro h
@@ -506,16 +507,16 @@ theorem inter_empty (A : St) : inter A empty =st empty := by
       exact hempty
     · intro h
       constructor
-      · /- mem x A -/
+      · /- St.mem x A -/
         exfalso
-        replace h := (mem_empty x).mp h
+        replace h := (St.mem_empty x).mp h
         exact h
       · exact h
 
-theorem inter_self (A : St) : inter A A =st A := by
-    apply (set_eq (inter A A) A).mp
+theorem St.inter_idem (A : St) : St.inter A A =st A := by
+    apply (St.ext (St.inter A A) A).mp
     intro x
-    rw [mem_inter]
+    rw [St.mem_inter]
 
     constructor
     · intro h
@@ -523,53 +524,53 @@ theorem inter_self (A : St) : inter A A =st A := by
       exact hA1
     · intro h
       constructor
-      · /- mem x A -/
+      · /- St.mem x A -/
         exact h
-      · /- mem x A -/
+      · /- St.mem x A -/
         exact h
 
 @[simp]
-theorem inter_comm (A B : St) : inter A B =st inter B A := by
-    apply (set_eq (inter A B) (inter B A)).mp
+theorem St.inter_comm (A B : St) : St.inter A B =st St.inter B A := by
+    apply (St.ext (St.inter A B) (St.inter B A)).mp
     intro x
-    rw [mem_inter]
-    rw [mem_inter]
+    rw [St.mem_inter]
+    rw [St.mem_inter]
 
     constructor
     · intro h
       obtain ⟨hA, hB⟩ := h
       constructor
-      · /- mem x B -/
+      · /- St.mem x B -/
         exact hB
-      · /- mem x A -/
+      · /- St.mem x A -/
         exact hA
     · intro h
       obtain ⟨hB, hA⟩ := h
       constructor
-      · /- mem x A -/
+      · /- St.mem x A -/
         exact hA
-      · /- mem x B -/
+      · /- St.mem x B -/
         exact hB
 
 @[simp]
-theorem inter_congr_left {A B C : St} (h : A =st B) :
-  inter C A =st inter C B := by
+theorem St.inter_congr_left {A B C : St} (h : A =st B) :
+  St.inter C A =st St.inter C B := by
 
   calc
-    inter C A =st inter A C := by apply inter_comm
-    _         =st inter B C := by apply inter_congr_right h
-    _         =st inter C B := by apply inter_comm
+    St.inter C A =st St.inter A C := by apply St.inter_comm
+    _         =st St.inter B C := by apply St.inter_congr_right h
+    _         =st St.inter C B := by apply St.inter_comm
 
 
-theorem inter_ass (A B C : St) :
-    inter (inter A B) C =st inter A (inter B C) := by
+theorem St.inter_ass (A B C : St) :
+    St.inter (St.inter A B) C =st St.inter A (St.inter B C) := by
 
-    apply (set_eq (inter (inter A B) C) (inter A (inter B C))).mp
+    apply (St.ext (St.inter (St.inter A B) C) (St.inter A (St.inter B C))).mp
     intro x
-    rw [mem_inter]
-    rw [mem_inter]
-    rw [mem_inter]
-    rw [mem_inter]
+    rw [St.mem_inter]
+    rw [St.mem_inter]
+    rw [St.mem_inter]
+    rw [St.mem_inter]
 
     constructor
     · intro h
@@ -592,16 +593,16 @@ theorem inter_ass (A B C : St) :
         · exact hB
       · exact hC
 
-theorem uni_distr_left (A B C : St) :
-    uni A (inter B C) =st inter (uni A B) (uni A C) := by
+theorem St.uni_distr_left (A B C : St) :
+    St.uni A (St.inter B C) =st St.inter (St.uni A B) (St.uni A C) := by
 
-    apply (set_eq (uni A (inter B C)) (inter (uni A B) (uni A C))).mp
+    apply (St.ext (St.uni A (St.inter B C)) (St.inter (St.uni A B) (St.uni A C))).mp
     intro x
-    rw [mem_uni]
-    rw [mem_inter]
-    rw [mem_inter]
-    rw [mem_uni]
-    rw [mem_uni]
+    rw [St.mem_uni]
+    rw [St.mem_inter]
+    rw [St.mem_inter]
+    rw [St.mem_uni]
+    rw [St.mem_uni]
 
     constructor
     · intro h
@@ -631,36 +632,41 @@ theorem uni_distr_left (A B C : St) :
           · exact hC
 
 
-theorem uni_distr_right (A B C : St) :
-    uni (inter B C) A =st inter (uni B A) (uni C A) := by
+theorem St.uni_distr_right (A B C : St) :
+    St.uni (St.inter B C) A =st St.inter (St.uni B A) (St.uni C A) := by
 
     calc
-      uni (inter B C) A
-        =st uni A (inter B C) := by apply uni_comm
+      St.uni (St.inter B C) A
+        =st St.uni A (St.inter B C) := by
+        apply St.uni_comm
 
-      _ =st inter (uni A B) (uni A C) := by apply uni_distr_left
+      _ =st St.inter (St.uni A B) (St.uni A C) := by
+        apply uni_distr_left
 
-      _ =st inter (uni B A) (uni A C) := by
+      _ =st St.inter (St.uni B A) (St.uni A C) := by
 
-        apply inter_congr_right
-        apply uni_comm
+        apply St.inter_congr_right
+        apply St.uni_comm
 
-      _ =st inter (uni B A) (uni C A) := by
+      _ =st St.inter (St.uni B A) (St.uni C A) := by
 
         apply inter_congr_left
-        apply uni_comm
+        apply St.uni_comm
 
 
-theorem inter_distr_left (A B C : St) :
-    inter A (uni B C) =st uni (inter A B) (inter A C) := by
+theorem St.inter_distr_left (A B C : St) :
+    St.inter A (St.uni B C) =st
+    St.uni (St.inter A B) (St.inter A C) := by
 
-    apply (set_eq (inter A (uni B C)) (uni (inter A B) (inter A C))).mp
+    apply (St.ext (St.inter A (St.uni B C))
+        (St.uni (St.inter A B) (St.inter A C))).mp
+
     intro x
-    rw [mem_inter]
-    rw [mem_uni]
-    rw [mem_uni]
-    rw [mem_inter]
-    rw [mem_inter]
+    rw [St.mem_inter]
+    rw [St.mem_uni]
+    rw [St.mem_uni]
+    rw [St.mem_inter]
+    rw [St.mem_inter]
 
     constructor
     · intro h
@@ -689,206 +695,226 @@ theorem inter_distr_left (A B C : St) :
           exact hC
 
 
-theorem inter_distr_right (A B C : St) :
-    inter (uni B C) A =st uni (inter B A) (inter C A) := by
+theorem St.inter_distr_right (A B C : St) :
+    St.inter (St.uni B C) A =st
+        St.uni (St.inter B A) (St.inter C A) := by
 
     calc
-      inter (uni B C) A
-        =st inter A (uni B C) := by apply inter_comm
+      St.inter (St.uni B C) A
+        =st St.inter A (St.uni B C) := by apply St.inter_comm
 
-      _ =st uni (inter A B) (inter A C) := by apply inter_distr_left
+      _ =st St.uni (St.inter A B) (St.inter A C) :=
+        by apply St.inter_distr_left
 
-      _ =st uni (inter B A) (inter A C) := by
+      _ =st St.uni (St.inter B A) (St.inter A C) := by
 
-        apply uni_congr_left
-        apply inter_comm
+        apply St.uni_congr_left
+        apply St.inter_comm
 
-      _ =st uni (inter B A) (inter C A) := by
+      _ =st St.uni (St.inter B A) (St.inter C A) := by
 
-        apply uni_congr_right
-        apply inter_comm
+        apply St.uni_congr_right
+        apply St.inter_comm
 
 
 /- Equality exercises -/
 
 
-theorem empty_not_singlet_empty :
-    (empty =st singlet empty) → False := by
+theorem St.empty_not_singlet_empty :
+    (St.empty =st St.singlet St.empty) → False := by
 
     intro h
-    replace h := (set_eq empty (singlet empty)).mpr h
-    replace h := h empty
+    replace h := (St.ext St.empty (St.singlet St.empty)).mpr h
+    replace h := h St.empty
 
-    apply (mem_empty empty).mp
+    apply (St.mem_empty St.empty).mp
     apply h.mpr
-    apply (mem_singlet empty empty).mpr
+    apply (St.mem_singlet St.empty St.empty).mpr
     rfl
 
-theorem empty_not_singlet_singlet_empty :
-    (empty =st singlet (singlet empty)) → False := by
+theorem St.empty_not_singlet_singlet_empty :
+    (St.empty =st St.singlet (St.singlet St.empty)) → False := by
 
     intro h
-    replace h := (set_eq empty (singlet (singlet empty))).mpr h
-    replace h := h (singlet empty)
+    replace h := (St.ext St.empty (
+        St.singlet (St.singlet St.empty))).mpr h
+    replace h := h (St.singlet St.empty)
 
-    apply (mem_empty (singlet empty)).mp
+    apply (St.mem_empty (St.singlet St.empty)).mp
     apply h.mpr
-    apply (mem_singlet (singlet empty) (singlet empty)).mpr
+    apply (St.mem_singlet (St.singlet St.empty)
+        (St.singlet St.empty)).mpr
     rfl
 
-theorem empty_not_pair_empty_singlet_empty :
-    (empty =st pair empty (singlet empty)) → False := by
+theorem St.empty_not_pair_empty_singlet_empty :
+    (St.empty =st St.pair St.empty (St.singlet St.empty)) → False := by
 
     intro h
-    replace h := (set_eq empty (pair empty (singlet empty))).mpr h
-    replace h := h empty
+    replace h := (St.ext St.empty (
+        St.pair St.empty (St.singlet St.empty))).mpr h
+    replace h := h St.empty
 
-    apply (mem_empty empty).mp
+    apply (St.mem_empty St.empty).mp
     apply h.mpr
-    apply (mem_pair empty (singlet empty) empty).mpr
+    apply (St.mem_pair St.empty (St.singlet St.empty) St.empty).mpr
 
     left
     rfl
 
-theorem singlet_empty_not_singlet_singlet_empty :
-  (singlet empty =st singlet (singlet empty)) → False := by
+theorem St.singlet_empty_not_singlet_singlet_empty :
+  (St.singlet St.empty =st
+    St.singlet (St.singlet St.empty)) → False := by
 
   intro h
-  apply empty_not_singlet_empty
-  apply (set_eq empty (singlet empty)).mp
+  apply St.empty_not_singlet_empty
+  apply (St.ext St.empty (St.singlet St.empty)).mp
   intro x
 
   replace h :=
-      (set_eq (singlet empty) (singlet (singlet empty))).mpr h
+      (St.ext (St.singlet St.empty)
+        (St.singlet (St.singlet St.empty))).mpr h
 
   constructor
   · intro hempty
-    replace hempty := (mem_empty x).mp hempty
+    replace hempty := (St.mem_empty x).mp hempty
     exfalso
     exact hempty
 
   · intro hxsingletempty
     replace hxsingletempty :=
-        (mem_singlet empty x).mp hxsingletempty
+        (St.mem_singlet St.empty x).mp hxsingletempty
 
-    have hemptyeqsingletempty : empty =st singlet empty := by
-        have hmememptysingletempty : mem empty (singlet empty) := by
-            apply (mem_singlet empty empty).mpr
+    have hemptyeqsingletempty : St.empty =st St.singlet St.empty := by
+        have hmememptysingletempty :
+            St.mem St.empty (St.singlet St.empty) := by
+
+            apply (St.mem_singlet St.empty St.empty).mpr
             rfl
 
-        --apply (set_eq empty (singlet empty)).mp
-        replace h := (h empty).mp hmememptysingletempty
-        apply (mem_singlet (singlet empty) empty).mp
+        --apply (St.ext St.empty (St.singlet St.empty)).mp
+        replace h := (h St.empty).mp hmememptysingletempty
+        apply (St.mem_singlet (St.singlet St.empty) St.empty).mp
         exact h
 
-    rw [mem_congr_right hemptyeqsingletempty]
+    rw [St.mem_congr_right hemptyeqsingletempty]
 
-    apply (mem_singlet empty x).mpr
+    apply (St.mem_singlet St.empty x).mpr
     exact hxsingletempty
 
-theorem singlet_empty_not_pair_empty_singlet_empty :
-  (singlet empty =st pair empty (singlet empty)) → False := by
+theorem St.singlet_empty_not_pair_empty_singlet_empty :
+  (St.singlet St.empty =st
+    St.pair St.empty (St.singlet St.empty)) → False := by
 
   intro h
-  apply empty_not_singlet_empty
-  apply (set_eq empty (singlet empty)).mp
+  apply St.empty_not_singlet_empty
+  apply (St.ext St.empty (St.singlet St.empty)).mp
   intro x
 
   replace h :=
-      (set_eq (singlet empty) (pair empty (singlet empty))).mpr h
+      (St.ext (St.singlet St.empty)
+        (St.pair St.empty (St.singlet St.empty))).mpr h
 
   constructor
   · intro hempty
-    replace hempty := (mem_empty x).mp hempty
+    replace hempty := (St.mem_empty x).mp hempty
     exfalso
     exact hempty
 
   · intro hxsingletempty
     replace hxsingletempty :=
-        (mem_singlet empty x).mp hxsingletempty
+        (St.mem_singlet St.empty x).mp hxsingletempty
 
-    have hemptyeqsingletempty : empty =st singlet empty := by
+    have hemptyeqsingletempty : St.empty =st St.singlet St.empty := by
         have hmemsingletemptypairemptysingletempty :
-            mem (singlet empty) (pair empty (singlet empty)) := by
-            apply (mem_pair empty (singlet empty) (singlet empty)).mpr
+            St.mem (St.singlet St.empty)
+                (St.pair St.empty (St.singlet St.empty)) := by
+
+            apply (St.mem_pair St.empty (
+                St.singlet St.empty) (St.singlet St.empty)).mpr
             right
             rfl
 
-        replace h := (h (singlet empty)).mpr
+        replace h := (h (St.singlet St.empty)).mpr
         replace h := h hmemsingletemptypairemptysingletempty
-        replace h := (mem_singlet empty (singlet empty)).mp h
-        replace h := eqst_symm h
+        replace h := (St.mem_singlet St.empty (
+            St.singlet St.empty)).mp h
+        replace h := St.eq_symm h
         exact h
 
-    rw [mem_congr_right hemptyeqsingletempty]
+    rw [St.mem_congr_right hemptyeqsingletempty]
 
-    apply (mem_singlet empty x).mpr
+    apply (St.mem_singlet St.empty x).mpr
     exact hxsingletempty
 
-theorem singlet_singlet_empty_not_pair_empty_singlet_empty :
-  (singlet (singlet empty) =st pair empty (singlet empty)) → False := by
+theorem St.singlet_singlet_empty_not_pair_empty_singlet_empty :
+  (St.singlet (St.singlet St.empty) =st
+    St.pair St.empty (St.singlet St.empty)) → False := by
 
   intro h
-  apply empty_not_singlet_empty
-  apply (set_eq empty (singlet empty)).mp
+  apply St.empty_not_singlet_empty
+  apply (St.ext St.empty (St.singlet St.empty)).mp
   intro x
 
   replace h :=
-      (set_eq (singlet (singlet empty))
-        (pair empty (singlet empty))).mpr h
+      (St.ext (St.singlet (St.singlet St.empty))
+        (St.pair St.empty (St.singlet St.empty))).mpr h
 
   constructor
   · intro hempty
-    replace hempty := (mem_empty x).mp hempty
+    replace hempty := (St.mem_empty x).mp hempty
     exfalso
     exact hempty
 
   · intro hxsingletempty
     replace hxsingletempty :=
-        (mem_singlet empty x).mp hxsingletempty
+        (St.mem_singlet St.empty x).mp hxsingletempty
 
     have hemptyeqsingletempty :
-        empty =st singlet empty := by
+        St.empty =st St.singlet St.empty := by
 
         have hmememptypairemptysingletempty :
-            mem empty (pair empty (singlet empty)) := by
-            apply (mem_pair empty (singlet empty) empty).mpr
+            St.mem St.empty (
+                St.pair St.empty (St.singlet St.empty)) := by
+
+            apply (St.mem_pair St.empty (
+                St.singlet St.empty) St.empty).mpr
             left
             rfl
 
-        replace h := (h empty).mpr
+        replace h := (h St.empty).mpr
         replace h := h hmememptypairemptysingletempty
-        replace h := (mem_singlet (singlet empty) empty).mp h
+        replace h := (St.mem_singlet (
+            St.singlet St.empty) St.empty).mp h
         exact h
 
-    rw [mem_congr_right hemptyeqsingletempty]
+    rw [St.mem_congr_right hemptyeqsingletempty]
 
-    apply (mem_singlet empty x).mpr
+    apply (St.mem_singlet St.empty x).mpr
     exact hxsingletempty
 
 
-theorem eqst_singlet {x y : St} (h : x =st y) :
-    singlet x =st singlet y := by
+theorem St.eq_singlet {x y : St} (h : x =st y) :
+    St.singlet x =st St.singlet y := by
 
-    apply (set_eq (singlet x) (singlet y)).mp
+    apply (St.ext (St.singlet x) (St.singlet y)).mp
 
     intro z
 
     constructor
     · intro hzSingletX
-      have hZeqX : z =st x := (mem_singlet x z).mp hzSingletX
+      have hZeqX : z =st x := (St.mem_singlet x z).mp hzSingletX
       have hZeqY : z =st y := by
         calc
             z =st x := hZeqX
             _ =st y := h
-      have hzSingletY := (mem_singlet y z).mpr hZeqY
+      have hzSingletY := (St.mem_singlet y z).mpr hZeqY
       exact hzSingletY
     · intro hzSingletY
-      have hZeqY : z =st y := (mem_singlet y z).mp hzSingletY
+      have hZeqY : z =st y := (St.mem_singlet y z).mp hzSingletY
       have hZeqX : z =st x := by
         calc
             z =st y := hZeqY
-            _ =st x := eqst_symm h
-      have hzSingletX := (mem_singlet x z).mpr hZeqX
+            _ =st x := St.eq_symm h
+      have hzSingletX := (St.mem_singlet x z).mpr hZeqX
       exact hzSingletX
 
