St/Nt.lean
@@ -1,6 +1,73 @@
 import St.Axioms
 
 
+/- Set succ Axioms -/
+
+
+axiom St.set_exists_succ (n : St) :
+    ∃ S : St, ∀ x : St, St.mem x S ↔ St.mem x (St.uni n (St.singlet n))
+
+noncomputable def St.set_succ (x : St) : St :=
+    Classical.choose (St.set_exists_succ x)
+
+theorem St.mem_succ (n : St) :
+  ∀ x : St, St.mem x (St.set_succ n) ↔
+    St.mem x (St.uni n (St.singlet n)) :=
+
+  Classical.choose_spec (St.set_exists_succ n)
+
+
+/- Set Nt definition -/
+
+
+axiom St.set_exists_infinity :
+    ∃ S : St, St.mem St.empty S ∧
+        ∀ y : St, St.mem y S → St.mem (St.set_succ y) S
+
+noncomputable def St.set_Inf : St :=
+    Classical.choose St.set_exists_infinity
+
+theorem St.mem_Inf :
+    St.mem St.empty St.set_Inf ∧
+        ∀ y : St, St.mem y St.set_Inf →
+            St.mem (St.set_succ y) St.set_Inf :=
+
+    Classical.choose_spec St.set_exists_infinity
+
+theorem St.mem_Inf_empty : St.mem St.empty set_Inf :=
+  mem_Inf.1
+
+theorem St.mem_Inf_succ (y : St) (h : St.mem y set_Inf) :
+  St.mem (St.set_succ y) set_Inf :=
+
+  St.mem_Inf.2 y h
+
+def St.is_Nt (x : St) : Prop := ∀ P : St → Prop,
+  P St.empty → (∀ n, P n → P (St.set_succ n)) → P x
+
+noncomputable def St.set_Nt : St :=
+    Classical.choose (set_exists_specification set_Inf St.is_Nt)
+
+theorem St.mem_set_Nt (x : St) : 
+  St.mem x set_Nt ↔ St.mem x set_Inf ∧ is_Nt x :=
+  Classical.choose_spec (set_exists_specification set_Inf is_Nt) x
+
+theorem St.set_Nt_induct (P : St → Prop)
+  (base : P St.empty)
+  (step : ∀ x, P x → P (St.set_succ x))
+  : ∀ x, St.mem x set_Nt → P x := by
+
+  intro x h_mem
+
+  rw [St.mem_set_Nt] at h_mem
+
+  let h_is_Nt := h_mem.2
+
+  apply h_is_Nt P
+  · exact base
+  · exact step
+
+
 /- Nt definition -/
 
 
@@ -8,7 +75,7 @@ axiom Nt : Type
 axiom Nt.zero : Nt
 axiom Nt.succ : Nt → Nt
 axiom Nt.eq : Nt → Nt → Prop
-notation:50 a " =nt " b => Nt.eq a b
+infix:50 " =nt " => Nt.eq
 
 axiom Nt.eq_rfl {a : Nt} : a =nt a
 axiom Nt.eq_symm {a b : Nt} : (a =nt b) → (b =nt a)
@@ -16,90 +83,25 @@ axiom Nt.eq_trans {a b c : Nt} : (a =nt b) → (b =nt c) → (a =nt c)
 instance : Trans Nt.eq Nt.eq Nt.eq where trans := Nt.eq_trans
 
 
-/- repr_Nt Axioms -/
+/- St.from_Nt Axioms -/
 
 
-axiom repr_Nt : Nt → St
+axiom St.from_Nt : Nt → St
 
-axiom repr_Nt_def (a b : Nt) :
-    (a =nt b) ↔ (repr_Nt a =st repr_Nt b)
+axiom St.from_Nt_eq (a b : Nt) :
+    (a =nt b) ↔ (St.from_Nt a =st St.from_Nt b)
 
-axiom mem_repr_Nt (n : Nt) :
-    mem (repr_Nt n) set_Nt
+axiom St.from_Nt_mem (n : Nt) :
+    St.mem (St.from_Nt n) St.set_Nt
 
-axiom repr_Nt_surj {x : St} :
-    mem x set_Nt → ∃ n : Nt, repr_Nt n =st x
+axiom Nt.from_St_mem {x : St} :
+    St.mem x St.set_Nt → ∃ n : Nt, St.from_Nt n =st x
 
-axiom zero_repr_Nt :
-    repr_Nt Nt.zero =st empty
+axiom St.from_Nt_zero :
+    St.from_Nt Nt.zero =st St.empty
 
-
-/- Succ Axioms -/
-
-
-axiom set_exists_succ (n : St) :
-    ∃ S : St, ∀ x : St, mem x S ↔ mem x (uni n (singlet n))
-
-noncomputable def set_succ (x : St) : St :=
-    Classical.choose (set_exists_succ x)
-
-theorem mem_succ (n : St) :
-  ∀ x : St, mem x (set_succ n) ↔ mem x (uni n (singlet n)) :=
-
-  Classical.choose_spec (set_exists_succ n)
-
-axiom succ_repr_Nt (n : Nt) :
-    repr_Nt (Nt.succ n) =st set_succ (repr_Nt n)
-
-
-/- set_Nt deifinition -/
-
-
-axiom set_exists_infinity :
-    ∃ S : St, mem empty S ∧
-        ∀ y : St, mem y S → mem (set_succ y) S
-
-noncomputable def set_Inf : St :=
-    Classical.choose set_exists_infinity
-
-theorem mem_Inf :
-    mem empty set_Inf ∧
-        ∀ y : St, mem y set_Inf → mem (set_succ y) set_Inf :=
-
-    Classical.choose_spec set_exists_infinity
-
-theorem mem_Inf_empty : mem empty set_Inf :=
-  mem_Inf.1
-
-theorem mem_Inf_succ (y : St) (h : mem y set_Inf) :
-  mem (set_succ y) set_Inf :=
-
-  mem_Inf.2 y h
-
-def is_Nt (x : St) : Prop := ∀ P : St → Prop,
-  P empty → (∀ n, P n → P (set_succ n)) → P x
-
-noncomputable def set_Nt : St :=
-    Classical.choose (set_exists_specification set_Inf is_Nt)
-
-theorem mem_set_Nt (x : St) : 
-  mem x set_Nt ↔ mem x set_Inf ∧ is_Nt x :=
-  Classical.choose_spec (set_exists_specification set_Inf is_Nt) x
-
-theorem set_Nt_induct (P : St → Prop)
-  (base : P empty)
-  (step : ∀ x, P x → P (set_succ x))
-  : ∀ x, mem x set_Nt → P x := by
-
-  intro x h_mem
-
-  rw [mem_set_Nt] at h_mem
-
-  let h_is_Nt := h_mem.2
-
-  apply h_is_Nt P
-  · exact base
-  · exact step
+axiom St.from_Nt_succ (n : Nt) :
+    St.from_Nt (Nt.succ n) =st St.set_succ (St.from_Nt n)
 
 
 /- Succ properties -/
@@ -110,55 +112,61 @@ theorem Nt.succ_ne_zero (n : Nt) :
 
   intro h
 
-  have h_st : set_succ (repr_Nt n) =st empty := calc
-    set_succ (repr_Nt n)
-    _ =st repr_Nt (Nt.succ n) := eqst_symm (succ_repr_Nt n)
-    _ =st repr_Nt Nt.zero     := (repr_Nt_def _ _).1 h
-    _ =st empty               := zero_repr_Nt
+  have h_st : St.set_succ (St.from_Nt n) =st St.empty := calc
+    St.set_succ (St.from_Nt n)
+    _ =st St.from_Nt (Nt.succ n) := St.eq_symm (St.from_Nt_succ n)
+    _ =st St.from_Nt Nt.zero     := (St.from_Nt_eq _ _).1 h
+    _ =st St.empty               := St.from_Nt_zero
 
-  have mem_self : mem (repr_Nt n) (set_succ (repr_Nt n)) := by
-    rw [mem_succ]
-    rw [mem_uni]
+  have hmem_self : St.mem (St.from_Nt n)
+    (St.set_succ (St.from_Nt n)) := by
+
+    rw [St.mem_succ]
+    rw [St.mem_uni]
     right
-    rw [mem_singlet]
+    rw [St.mem_singlet]
 
-  rw [mem_congr_right h_st] at mem_self
-  rw [mem_empty] at mem_self
-  exact mem_self
+  rw [St.mem_congr_right h_st] at hmem_self
+  rw [St.mem_empty] at hmem_self
+  exact hmem_self
 
-axiom set_succ_inj {A B : St} : (set_succ A =st set_succ B) → (A =st B)
+axiom St.set_succ_inj {A B : St} :
+    (St.set_succ A =st St.set_succ B) → (A =st B)
 
 theorem Nt.succ_inj {a b : Nt} (h : (Nt.succ a =nt Nt.succ b)) :
   a =nt b := by
 
-  have h_st : set_succ (repr_Nt a) =st set_succ (repr_Nt b) := calc
-    set_succ (repr_Nt a)
-    _ =st repr_Nt (Nt.succ a) := eqst_symm (succ_repr_Nt a)
-    _ =st repr_Nt (Nt.succ b) := (repr_Nt_def _ _).1 h
-    _ =st set_succ (repr_Nt b) := succ_repr_Nt b
+  have h_st : St.set_succ (St.from_Nt a) =st
+    St.set_succ (St.from_Nt b) :=
 
-  have h_repr_eq : repr_Nt a =st repr_Nt b :=
-    set_succ_inj h_st
+    calc
+        St.set_succ (St.from_Nt a)
+        _ =st St.from_Nt (Nt.succ a) := St.eq_symm (St.from_Nt_succ a)
+        _ =st St.from_Nt (Nt.succ b) := (St.from_Nt_eq _ _).1 h
+        _ =st St.set_succ (St.from_Nt b) := St.from_Nt_succ b
 
-  exact (repr_Nt_def a b).2 h_repr_eq
+  have h_repr_eq : St.from_Nt a =st St.from_Nt b :=
+    St.set_succ_inj h_st
 
-axiom set_succ_congr {A B : St} :
-    (A =st B) → (set_succ A =st set_succ B)
+  exact (St.from_Nt_eq a b).2 h_repr_eq
+
+axiom St.set_succ_congr {A B : St} :
+    (A =st B) → (St.set_succ A =st St.set_succ B)
 
 theorem Nt.succ_congr {a b : Nt} :
   (a =nt b) → ((Nt.succ a) =nt (Nt.succ b)) := by
 
   intro h
 
-  have h_st : repr_Nt a =st repr_Nt b := (repr_Nt_def a b).1 h
+  have h_st : St.from_Nt a =st St.from_Nt b := (St.from_Nt_eq a b).1 h
 
-  apply (repr_Nt_def _ _).2
+  apply (St.from_Nt_eq _ _).2
 
   calc
-    repr_Nt (Nt.succ a)
-    _ =st set_succ (repr_Nt a) := succ_repr_Nt a
-    _ =st set_succ (repr_Nt b) := set_succ_congr h_st
-    _ =st repr_Nt (Nt.succ b)  := eqst_symm (succ_repr_Nt b)
+    St.from_Nt (Nt.succ a)
+    _ =st St.set_succ (St.from_Nt a) := St.from_Nt_succ a
+    _ =st St.set_succ (St.from_Nt b) := St.set_succ_congr h_st
+    _ =st St.from_Nt (Nt.succ b)  := St.eq_symm (St.from_Nt_succ b)
 
 
 /- Nt Induction -/
@@ -174,15 +182,15 @@ theorem Nt.induction (P : Nt → Prop)
 
   intro n
 
-  let Q := λ (x : St) => ∃ (k : Nt), (repr_Nt k =st x) ∧ P k
+  let Q := λ (x : St) => ∃ (k : Nt), ((St.from_Nt k) =st x) ∧ P k
 
-  have q_base : Q empty := by
+  have q_base : Q St.empty := by
     exists Nt.zero
     constructor
-    · exact zero_repr_Nt
+    · exact St.from_Nt_zero
     · exact base
 
-  have q_step : ∀ (x : St), Q x → Q (set_succ x) := by
+  have q_step : ∀ (x : St), Q x → Q (St.set_succ x) := by
     intro x h_qx
     rcases h_qx with ⟨k, h_repr_k_eq_x, h_Pk⟩
     exists (Nt.succ k)
@@ -190,21 +198,21 @@ theorem Nt.induction (P : Nt → Prop)
     constructor
     ·
       calc
-        repr_Nt (Nt.succ k)
-        _ =st set_succ (repr_Nt k) := succ_repr_Nt k
-        _ =st set_succ x           := set_succ_congr h_repr_k_eq_x
+        St.from_Nt (Nt.succ k)
+        _ =st St.set_succ (St.from_Nt k) := St.from_Nt_succ k
+        _ =st St.set_succ x           := St.set_succ_congr h_repr_k_eq_x
 
     ·
       apply step k
       exact h_Pk
 
-  have h_Q_n : Q (repr_Nt n) := by
-    apply set_Nt_induct Q q_base q_step
-    exact mem_repr_Nt n
+  have h_Q_n : Q (St.from_Nt n) := by
+    apply St.set_Nt_induct Q q_base q_step
+    exact St.from_Nt_mem n
 
   rcases h_Q_n with ⟨k, h_repr_eq, h_Pk⟩
 
   apply Nt.prop_congr _ h_Pk
 
-  apply (repr_Nt_def k n).2
+  apply (St.from_Nt_eq k n).2
   exact h_repr_eq
