St.lean
@@ -5,4 +5,6 @@ import St.Russell
 import St.Nt
 import St.Addition
 import St.Order
--- import St.Function
+import St.Multiplication
+import St.Composition
+import St.Bijection
