St/Axioms.lean
@@ -1,27 +1,27 @@
 import St.Subset
 
-axiom prop_congr {x y : St} {P : St → Prop} (h : x =st y) :
+axiom St.prop_congr {x y : St} {P : St → Prop} (h : x =st y) :
   P x ↔ P y
 
-axiom mem_congr_left {x y A : St} (h : x =st y) :
-  mem x A ↔ mem y A
+axiom St.mem_congr_left {x y A : St} (h : x =st y) :
+  St.mem x A ↔ St.mem y A
 
 
-axiom set_exists_replacement (A : St) (P : St → St → Prop)
-    (h: ∀ x y1 y2 : St, mem x A → P x y1 → P x y2 → (y1 =st y2)) :
+axiom St.set_exists_replacement (A : St) (P : St → St → Prop)
+    (h: ∀ x y1 y2 : St, St.mem x A → P x y1 → P x y2 → (y1 =st y2)) :
 
     ∃ S : St,
-        ∀ z : St, mem z S ↔ (∃ x : St, mem x A ∧ (P x z))
+        ∀ z : St, St.mem z S ↔ (∃ x : St, St.mem x A ∧ (P x z))
 
 
-theorem set_exists_specification (A : St) (P : St → Prop) :
+theorem St.set_exists_specification (A : St) (P : St → Prop) :
     ∃ S : St,
-        ∀ y : St, mem y S ↔ (mem y A ∧ (P y)) := by
+        ∀ y : St, St.mem y S ↔ (St.mem y A ∧ (P y)) := by
 
     let PR (x y : St) : Prop := P x ∧ (y =st x)
 
     have hSuniq : (∀ x y1 y2 : St,
-        mem x A → (PR x y1) → (PR x y2) → (y1 =st y2)) := by
+        St.mem x A → (PR x y1) → (PR x y2) → (y1 =st y2)) := by
 
         intro x y1 y2 hxA hPy1 hPy2
         obtain ⟨hPx, hy1x⟩ := hPy1
@@ -29,10 +29,10 @@ theorem set_exists_specification (A : St) (P : St → Prop) :
 
         calc
             y1 =st x  := by apply hy1x
-            _  =st y2 := by apply (eqst_symm hy2x)
+            _  =st y2 := by apply (St.eq_symm hy2x)
 
 
-    obtain ⟨S, hS⟩ := set_exists_replacement A PR hSuniq
+    obtain ⟨S, hS⟩ := St.set_exists_replacement A PR hSuniq
 
     exists S
 
@@ -40,7 +40,7 @@ theorem set_exists_specification (A : St) (P : St → Prop) :
 
     constructor
     · intro hmemyS
-      have hexistsx : ∃ (x : St), mem x A ∧ PR x y := by
+      have hexistsx : ∃ (x : St), St.mem x A ∧ PR x y := by
         apply ((hS y).mp hmemyS)
 
       obtain ⟨x, hx⟩ := hexistsx
@@ -48,8 +48,8 @@ theorem set_exists_specification (A : St) (P : St → Prop) :
       obtain ⟨hPx, hxeqy⟩ := hPRxy
 
       constructor
-      · have hymemA : mem y A :=
-          (mem_congr_left (A := A) hxeqy).mpr hxmemA
+      · have hymemA : St.mem y A :=
+          (St.mem_congr_left (A := A) hxeqy).mpr hxmemA
 
         exact hymemA
 
@@ -67,47 +67,47 @@ theorem set_exists_specification (A : St) (P : St → Prop) :
         · exact hPy
         · rfl
 
-axiom set_regularity (A : St) (h : (A =st empty) → False) :
-    ∃ (x : St), mem x A ∧ (inter x A =st empty)
+axiom St.set_regularity (A : St) (h : (A =st St.empty) → False) :
+    ∃ (x : St), St.mem x A ∧ (St.inter x A =st St.empty)
 
 
-theorem set_not_self_member (A : St) : mem A A → False := by
+theorem St.set_not_self_member (A : St) : St.mem A A → False := by
 
     intro hAA
 
-    have hsingletAnotEmpty : (singlet A =st empty) → False := by
+    have hsingletAnotEmpty : (St.singlet A =st empty) → False := by
 
         intro hsingletAempty
-        apply (mem_empty A).mp
-        rw [← (mem_congr_right hsingletAempty)]
-        apply (mem_singlet A A).mpr
+        apply (St.mem_empty A).mp
+        rw [← (St.mem_congr_right hsingletAempty)]
+        apply (St.mem_singlet A A).mpr
         rfl
 
-    have hreg := set_regularity (singlet A) hsingletAnotEmpty
+    have hreg := St.set_regularity (St.singlet A) hsingletAnotEmpty
     obtain ⟨x, hx⟩ := hreg
     obtain ⟨hxmemsingletA, hxintersingletA⟩ := hx
     replace hxmemsingletA :=
-        (mem_singlet A x).mp hxmemsingletA
+        (St.mem_singlet A x).mp hxmemsingletA
     replace hxintersingletA :=
-        (set_eq (inter x (singlet A)) empty).mpr hxintersingletA
+        (St.ext (St.inter x (St.singlet A)) empty).mpr hxintersingletA
 
-    apply (mem_empty x).mp
+    apply (St.mem_empty x).mp
     apply (hxintersingletA x).mp
-    apply (mem_inter x (singlet A) x).mpr
+    apply (St.mem_inter x (St.singlet A) x).mpr
     constructor
-    · rw [(mem_congr_left hxmemsingletA)]
-      rw [(mem_congr_right hxmemsingletA)]
+    · rw [(St.mem_congr_left hxmemsingletA)]
+      rw [(St.mem_congr_right hxmemsingletA)]
       exact hAA
-    · apply (mem_singlet A x).mpr
+    · apply (St.mem_singlet A x).mpr
       apply hxmemsingletA
 
-theorem set_not_both_members (A B : St) :
-    (mem A B → False) ∨ (mem B A → False) := by
+theorem St.set_not_both_members (A B : St) :
+    (St.mem A B → False) ∨ (St.mem B A → False) := by
 
     apply Classical.not_not.mp
     intro h
 
-    have hmorgan : mem A B ∧ mem B A := by
+    have hmorgan : St.mem A B ∧ St.mem B A := by
         constructor
         · apply Classical.not_not.mp
           intro hAB
@@ -124,60 +124,60 @@ theorem set_not_both_members (A B : St) :
           apply hBA
           exact hright
 
-    have hpairABnotEmpty : (pair A B =st empty) → False := by
+    have hpairABnotEmpty : (St.pair A B =st empty) → False := by
 
         intro hpairABempty
         replace hpairABempty :=
-            (set_eq (pair A B) empty).mpr hpairABempty
-        apply (mem_empty A).mp
+            (St.ext (St.pair A B) empty).mpr hpairABempty
+        apply (St.mem_empty A).mp
         apply (hpairABempty A).mp
-        apply (mem_pair A B A).mpr
+        apply (St.mem_pair A B A).mpr
         left
         rfl
 
-    have hreg := set_regularity (pair A B) hpairABnotEmpty
+    have hreg := St.set_regularity (St.pair A B) hpairABnotEmpty
 
     obtain ⟨hAmemB, hBmemA⟩ := hmorgan
     obtain ⟨x, hx⟩ := hreg
     obtain ⟨hxmempairAB, hxinterpairAB⟩ := hx
     replace hxinterpairAB :=
-        (set_eq (inter x (pair A B)) empty).mpr hxinterpairAB
+        (St.ext (St.inter x (St.pair A B)) empty).mpr hxinterpairAB
 
-    replace hxmempairAB := (mem_pair A B x).mp hxmempairAB
+    replace hxmempairAB := (St.mem_pair A B x).mp hxmempairAB
     rcases hxmempairAB with hxA | hxB
     · 
-      apply (mem_empty B).mp
+      apply (St.mem_empty B).mp
       apply (hxinterpairAB B).mp
-      apply (mem_inter x (pair A B) B).mpr
+      apply (St.mem_inter x (St.pair A B) B).mpr
       constructor
       · 
-        rw [(mem_congr_right hxA)]
+        rw [(St.mem_congr_right hxA)]
         exact hBmemA
       ·
-        apply (mem_pair A B B).mpr
+        apply (St.mem_pair A B B).mpr
         right
         rfl
     · 
-      apply (mem_empty A).mp
+      apply (St.mem_empty A).mp
       apply (hxinterpairAB A).mp
-      apply (mem_inter x (pair A B) A).mpr
+      apply (St.mem_inter x (St.pair A B) A).mpr
       constructor
       · 
-        rw [(mem_congr_right hxB)]
+        rw [(St.mem_congr_right hxB)]
         exact hAmemB
       ·
-        apply (mem_pair A B A).mpr
+        apply (St.mem_pair A B A).mpr
         left
         rfl
 
 
-theorem set_universal_equivalence :
-    (∀ P : St → Prop, ∃ S : St, ∀ y : St, mem y S ↔ P y)
+theorem St.set_universal_equivalence :
+    (∀ P : St → Prop, ∃ S : St, ∀ y : St, St.mem y S ↔ P y)
     ↔
-    (∃ S : St, ∀ y : St, mem y S) := by
+    (∃ S : St, ∀ y : St, St.mem y S) := by
 
     constructor
-    · 
+    ·
       intro huniversalSpec
       let P (y : St) : Prop := y =st y
       obtain ⟨S, hS⟩ := huniversalSpec P
@@ -185,7 +185,7 @@ theorem set_universal_equivalence :
       intro y
       apply (hS y).mpr
       rfl
-    · 
+    ·
       intro huniversalSet
       obtain ⟨S, hS⟩ := huniversalSet
       intro P
@@ -194,7 +194,7 @@ theorem set_universal_equivalence :
       exists A
       intro y
       constructor
-      · 
+      ·
         intro hymemA
         obtain ⟨hymemS, hPy⟩ := (hA y).mp hymemA
         apply hPy
