St/Bijection.lean
@@ -1,0 +1,594 @@
+import St.Composition
+
+
+def Func.bij {A B : St} (f : Func A B) : Prop :=
+    Func.inj f ∧ Func.onto f
+
+axiom Func.exists_from_rel {A B : St} (P : St → St → Prop)
+  (h_tot : ∀ x : St, St.mem x A → ∃ y, St.mem y B ∧ P x y)
+  (h_uniq : ∀ x y1 y2 : St, St.mem x A → St.mem y1 B → St.mem y2 B →
+    P x y1 → P x y2 → (y1 =st y2)) :
+
+    ∃ f : Func A B, ∀ x, (hxmemA : St.mem x A) →
+        Func.app f x =st Classical.choose (h_tot x hxmemA)
+
+noncomputable def Func.from_rel {A B :St} (P : St → St → Prop)
+  (h_tot : ∀ x : St, St.mem x A → ∃ y, St.mem y B ∧ P x y)
+  (h_uniq : ∀ x y1 y2 : St, St.mem x A → St.mem y1 B → St.mem y2 B →
+    P x y1 → P x y2 → (y1 =st y2)) : Func A B :=
+
+    Classical.choose (Func.exists_from_rel P h_tot h_uniq)
+
+theorem Func.app_from_rel {A B : St} (P : St → St → Prop)
+  (h_tot : ∀ x : St, St.mem x A → ∃ y, St.mem y B ∧ P x y)
+  (h_uniq : ∀ x y1 y2 : St, St.mem x A → St.mem y1 B → St.mem y2 B →
+    P x y1 → P x y2 → (y1 =st y2)) :
+
+    ∀ x, (hxmemA : St.mem x A) →
+        Func.app (Func.from_rel P h_tot h_uniq) x =st
+            Classical.choose (h_tot x hxmemA)
+    :=
+
+    Classical.choose_spec (Func.exists_from_rel P h_tot h_uniq)
+
+axiom Func.exists_inv {A B : St}
+    (f : Func A B) (hfbij : Func.bij f) :
+
+    ∃ f' : Func B A,
+        ∀ x y : St, St.mem x A → St.mem y B →
+            y =st Func.app f x → x =st Func.app f' y
+
+noncomputable def Func.inv {A B : St}
+    (f : Func A B) (hfbij : Func.bij f) : Func B A :=
+
+    Classical.choose (Func.exists_inv f hfbij)
+
+theorem Func.app_inv {A B : St} (f : Func A B) (hfbij : Func.bij f) :
+
+    ∀ x y : St, St.mem x A → St.mem y B →
+        y =st Func.app f x →
+            x =st Func.app (Func.inv f hfbij) y :=
+
+    Classical.choose_spec (Func.exists_inv f hfbij)
+
+axiom Func.bij_congr {A B : St} {f g : Func A B} :
+
+    (f =func g) → (Func.bij f ↔ Func.bij g)
+
+axiom Func.inv_congr_left {A B : St}
+    {f g : Func A B} {hfbij : Func.bij f} :
+
+    (hfeqg : f =func g) →
+
+        let hgbij := (Func.bij_congr hfeqg).mp hfbij
+        Func.inv f hfbij =func Func.inv g hgbij
+
+
+theorem Func.empty_empty_bijective (f : Func St.empty St.empty) :
+    Func.bij f := by
+
+    constructor
+    · apply (Func.empty_inj f)
+
+    · apply (Func.is_onto f).mpr
+      intro y hymemEmp
+
+      exfalso
+      apply (St.mem_empty y).mp
+      exact hymemEmp
+
+
+theorem Func.canc_bij_ff' {A B : St} (f : Func A B)
+    (f' : Func B A) (hfbij : Func.bij f) :
+
+    f' =func Func.inv f hfbij →
+        ∀ y, St.mem y B →
+            Func.app f (Func.app f' y) =st y := by
+
+    intro hf'eqfinv y hymemB
+
+    have ⟨hfinj, hfonto⟩ := hfbij
+
+    have ⟨x, hxmemA, hyeqfx⟩ := (Func.is_onto f).mp hfonto y hymemB
+
+    have hxeqf'y := Func.app_inv f hfbij x y hxmemA hymemB hyeqfx
+ 
+    calc
+        Func.app f (Func.app f' y)
+            =st Func.app f (Func.app (Func.inv f hfbij) y)
+                := Func.app_congr_right (
+                    Func.app_congr_left hf'eqfinv)
+
+        _   =st Func.app f x
+                := Func.app_congr_right (St.eq_symm hxeqf'y)
+
+        _   =st y
+                := St.eq_symm hyeqfx
+
+
+theorem Func.canc_bij_f'f {A B : St} (f : Func A B) (f' : Func B A)
+    (hfbij : Func.bij f) :
+
+    f' =func Func.inv f hfbij →
+        ∀ x, St.mem x A →
+            Func.app f' (Func.app f x) =st x := by
+
+    intro hf'eqfinv x hxmemA
+
+    have ⟨hfinj, hfonto⟩ := hfbij
+
+    have ⟨y, hymemB, hyeqfx⟩ := Func.tot f x hxmemA
+
+    have hxeqf'y := Func.app_inv f hfbij x y hxmemA hymemB hyeqfx
+
+    calc
+        Func.app f' (Func.app f x)
+            =st Func.app f' y
+                := Func.app_congr_right (St.eq_symm hyeqfx)
+
+        _   =st Func.app (Func.inv f hfbij) y
+                := Func.app_congr_left hf'eqfinv
+
+        _   =st x
+                := St.eq_symm hxeqf'y
+
+
+
+theorem Func.inv_bij {A B : St} (f: Func A B) (f' : Func B A)
+    (hfbij : Func.bij f) (hf'eqfinv : f' =func Func.inv f hfbij) :
+
+    Func.bij f' := by
+
+    have ⟨hfinj, hfonto⟩ := hfbij
+
+    constructor
+    · apply (Func.is_inj f').mpr
+      intro y y' hymemB hy'memB hf'yeqf'y'
+
+      calc
+        y =st Func.app f (Func.app f' y)
+            := St.eq_symm (
+                Func.canc_bij_ff' f f' hfbij hf'eqfinv y hymemB)
+
+        _ =st Func.app f (Func.app f' y')
+            := Func.app_congr_right hf'yeqf'y'
+
+        _ =st y'
+            := Func.canc_bij_ff' f f' hfbij hf'eqfinv y' hy'memB
+
+    · apply (Func.is_onto f').mpr
+      intro x hxmemA
+
+      have ⟨y, hymemB, hyeqfx⟩ := Func.tot f x hxmemA
+
+      exists y
+
+      constructor
+      · exact hymemB
+      · calc
+            x =st Func.app f' (Func.app f x)
+                := St.eq_symm (
+                    Func.canc_bij_f'f f f' hfbij hf'eqfinv x hxmemA)
+
+            _ =st Func.app f' y
+                := Func.app_congr_right (St.eq_symm hyeqfx)
+
+
+theorem Func.inv_f'_eq_f {A B : St} (f: Func A B) (f' : Func B A)
+    (hfbij : Func.bij f) (hf'eqfinv : f' =func Func.inv f hfbij)
+    (hf'bij : Func.bij f' := Func.inv_bij f f' hfbij hf'eqfinv) :
+
+    f =func (Func.inv f' hf'bij) := by
+
+    apply (Func.ext f (Func.inv f' hf'bij)).mp
+
+    intro x hxmemA
+
+    have ⟨y, hymemB, hyeqfx⟩ := Func.tot f x hxmemA
+
+    have hxeqf'y :=
+        Func.app_inv f hfbij x y hxmemA hymemB hyeqfx
+
+    have hfinvbij : Func.bij (Func.inv f hfbij) :=
+        (Func.bij_congr hf'eqfinv).mp hf'bij
+
+    have hyeqf''x :=
+        Func.app_inv (Func.inv f hfbij) hfinvbij y x
+            hymemB hxmemA hxeqf'y
+
+    calc
+        Func.app f x
+            =st y
+                := St.eq_symm hyeqfx
+
+        _   =st Func.app (Func.inv (Func.inv f hfbij) hfinvbij) x
+                := hyeqf''x
+
+        _   =st Func.app (Func.inv f' hf'bij) x
+                := Func.app_congr_left (
+                    Func.inv_congr_left (
+                        Func.eq_symm hf'eqfinv))
+
+
+theorem Func.comp_bij_if_fg_bij {A B C : St}
+    (f : Func A B) (g : Func B C)
+    (hfbij : Func.bij f) (hgbij : Func.bij g) :
+
+    Func.bij (Func.comp g f) := by
+
+    have ⟨hfinj, hfonto⟩ := hfbij
+    have ⟨hginj, hgonto⟩ := hgbij
+
+    have hgfinj := Func.comp_inj f g hfinj hginj
+    have hgfonto := Func.comp_onto f g hfonto hgonto
+
+    constructor
+    · exact hgfinj
+    · exact hgfonto
+
+
+
+theorem comp_inv_eq_f_inv_g_inv {A B C : St}
+    (f : Func A B) (g : Func B C)
+    (hfbij : Func.bij f) (hgbij : Func.bij g)
+    (hgfbij : Func.bij (Func.comp g f) :=
+        Func.comp_bij_if_fg_bij f g hfbij hgbij) :
+
+    Func.inv (Func.comp g f) hgfbij =func
+        Func.comp (Func.inv f hfbij) (Func.inv g hgbij) := by
+
+    let g' := (Func.inv g hgbij)
+    let f' := (Func.inv f hfbij)
+    let «(gf)'» := (Func.inv (Func.comp g f) hgfbij)
+
+    have hf'eqfinv : f' =func Func.inv f hfbij := by rfl
+    have hf'bij := Func.inv_bij f f' hfbij hf'eqfinv
+
+    have hg'eqginv : g' =func Func.inv g hgbij := by rfl
+    have hg'bij := Func.inv_bij g g' hgbij hg'eqginv
+
+    apply (Func.ext «(gf)'» (Func.comp f' g')).mp
+
+    intro z hzmemC
+
+    have ⟨hgfinj, hgfonto⟩ := hgfbij
+
+    have ⟨x, hxmemA, hzeqgfx⟩ :=
+        (Func.is_onto (Func.comp g f)).mp hgfonto z hzmemC
+
+    have «hxeq(gf)'z» :=
+        Func.app_inv (Func.comp g f) hgfbij x z hxmemA hzmemC hzeqgfx
+
+    have ⟨y, hymemB, hyeqfx⟩ := Func.tot f x hxmemA
+
+    have ⟨z', hz'memC, hz'eqgy⟩ := Func.tot g y hymemB
+
+    have hxeqf'y := Func.app_inv f hfbij x y hxmemA hymemB hyeqfx
+
+    have hyeqg'z' := Func.app_inv g hgbij y z' hymemB hz'memC hz'eqgy
+
+    have hzeqz' : z =st z' := by
+        calc
+            z =st Func.app (Func.comp g f) x
+                := hzeqgfx
+
+            _ =st Func.app g (Func.app f x)
+                := Func.app_comp f g hxmemA
+
+            _ =st Func.app g (Func.app f (Func.app f' y))
+                := Func.app_congr_right (
+                    Func.app_congr_right hxeqf'y)
+
+            _ =st Func.app g y
+                := Func.app_congr_right (
+                    Func.canc_bij_ff' f f' hfbij hf'eqfinv y hymemB)
+
+            _ =st Func.app g (Func.app g' z')
+                := Func.app_congr_right hyeqg'z'
+
+            _ =st z'
+                := Func.canc_bij_ff' g g' hgbij hg'eqginv z' hz'memC
+
+    calc
+        Func.app «(gf)'» z
+            =st x
+                := St.eq_symm «hxeq(gf)'z»
+
+        _   =st Func.app f' y
+                := hxeqf'y
+
+        _   =st Func.app f' (Func.app g' z')
+                := Func.app_congr_right hyeqg'z'
+
+        _   =st Func.app f' (Func.app g' z)
+                := Func.app_congr_right (
+                    Func.app_congr_right (
+                        St.eq_symm hzeqz'))
+
+        _   =st Func.app (Func.comp f' g') z
+                := St.eq_symm (Func.app_comp g' f' hzmemC)
+
+
+theorem Func.comp_incl_from_incl {A B C : St}
+    (hAsubB : St.subset A B) (hBsubC : St.subset B C)
+    (hAsubC : St.subset A C := St.subset_trans A B C hAsubB hBsubC) :
+
+    Func.comp (Func.incl B C hBsubC) (Func.incl A B hAsubB) =func
+        Func.incl A C  hAsubC := by
+
+    let f := Func.incl A B hAsubB
+    let g := Func.incl B C hBsubC
+    let h := Func.incl A C hAsubC
+
+    apply (Func.ext (Func.comp g f) h).mp
+    intro x hxmemA
+
+    have hxmemB : St.mem x B := (St.mem_subset A B).mp hAsubB x hxmemA
+
+    calc
+        Func.app (Func.comp g f) x
+
+            =st Func.app g (Func.app f x)
+                := Func.app_comp f g hxmemA
+
+        _   =st Func.app g x
+                := Func.app_congr_right (
+                    Func.app_incl hAsubB x hxmemA)
+
+        _   =st x
+                := Func.app_incl hBsubC x hxmemB
+
+        _   =st Func.app h x
+                := St.eq_symm (Func.app_incl hAsubC x hxmemA)
+
+theorem Func.comp_dom_identity {A B : St} (f : Func A B)
+    (hAsubA : St.subset A A := St.subset_rfl A) :
+
+    Func.comp f (Func.incl A A hAsubA) =func f := by
+
+    let i := (Func.incl A A hAsubA)
+
+    apply (Func.ext (Func.comp f i) f).mp
+    intro x hxmemA
+
+    calc
+        Func.app (Func.comp f i) x
+
+            =st Func.app f (Func.app i x)
+                := Func.app_comp i f hxmemA
+
+        _   =st Func.app f x
+                := Func.app_congr_right (
+                    Func.app_incl hAsubA x hxmemA)
+
+
+theorem Func.comp_codom_identity {A B : St} (f : Func A B)
+    (hBsubB : St.subset B B := St.subset_rfl B) :
+
+    Func.comp (Func.incl B B hBsubB) f =func f := by
+
+    let i := (Func.incl B B hBsubB)
+
+    apply (Func.ext (Func.comp i f) f).mp
+    intro x hxmemA
+
+    have ⟨y, hymemB, hyeqfx⟩ := Func.tot f x hxmemA
+
+    calc
+        Func.app (Func.comp i f) x
+
+        _   =st Func.app i (Func.app f x)
+                := Func.app_comp f i hxmemA
+
+        _   =st Func.app i y
+                := Func.app_congr_right (St.eq_symm hyeqfx)
+
+        _   =st y
+                := Func.app_incl hBsubB y hymemB
+
+        _   =st Func.app f x
+                := hyeqfx
+
+
+theorem Func.dom_identity_from_bij {A B : St}
+    (f : Func A B) (hfbij : Func.bij f)
+    (hAsubA : St.subset A A := St.subset_rfl A) :
+
+    Func.comp (Func.inv f hfbij) f =func Func.incl A A hAsubA := by
+
+    let f' := Func.inv f hfbij
+    have hf'eqfinv : f' =func Func.inv f hfbij := by rfl
+
+    let i := Func.incl A A hAsubA
+
+    apply (Func.ext (Func.comp f' f) i).mp
+    intro x hxmemA
+
+    calc
+        Func.app (Func.comp f' f) x
+            =st Func.app f' (Func.app f x)
+                := Func.app_comp f f' hxmemA
+
+        _   =st x
+                := Func.canc_bij_f'f f f' hfbij hf'eqfinv x hxmemA
+
+        _   =st Func.app i x
+                := St.eq_symm (Func.app_incl hAsubA x hxmemA)
+
+
+theorem Func.codom_identity_from_bij {A B : St}
+    (f : Func A B) (hfbij : Func.bij f)
+    (hBsubB : St.subset B B := St.subset_rfl B) :
+
+    Func.comp f (Func.inv f hfbij) =func Func.incl B B hBsubB := by
+
+    let f' := Func.inv f hfbij
+    have hf'eqfinv : f' =func Func.inv f hfbij := by rfl
+
+    let i := Func.incl B B hBsubB
+
+    apply (Func.ext (Func.comp f f') i).mp
+    intro y hymemB
+
+    calc
+        Func.app (Func.comp f f') y
+            =st Func.app f (Func.app f' y)
+                := Func.app_comp f' f hymemB
+
+        _   =st y
+                := Func.canc_bij_ff' f f' hfbij hf'eqfinv y hymemB
+
+        _   =st Func.app i y
+                := St.eq_symm (Func.app_incl hBsubB y hymemB)
+
+
+
+theorem Func.unique_piecewise_function {A B C : St}
+    (hAinterBempty : St.inter A B =st St.empty)
+    (f : Func A C) (g : Func B C)
+    (hAsubAB : St.subset A (St.uni A B) := St.subset_of_uni_left A B)
+    (hBsubAB : St.subset B (St.uni A B) := St.subset_of_uni_right A B) :
+
+    let iA := Func.incl A (St.uni A B) hAsubAB
+    let iB := Func.incl B (St.uni A B) hBsubAB
+    let piecewise_comps (h : Func (St.uni A B) C) :=
+        (Func.comp h iA =func f ∧ Func.comp h iB =func g)
+
+    ∃ h : Func (St.uni A B) C, piecewise_comps h ∧
+        ∀ h' : Func (St.uni A B) C, piecewise_comps h' → h' =func h
+
+    := by
+
+    intro iA iB piecewise_comps
+
+    let h := Func.piecewise f g
+
+    have hpiecewise_compsh : piecewise_comps h := by
+      constructor
+      · apply (Func.ext (Func.comp h iA) f).mp
+        intro x hxmemA
+        calc
+          Func.app (Func.comp h iA) x
+
+              =st Func.app h (Func.app iA x)
+                  := Func.app_comp iA h hxmemA
+
+          _   =st Func.app h x
+                  := Func.app_congr_right (
+                      Func.app_incl hAsubAB x hxmemA)
+
+          _   =st Func.app f x
+                  := Func.app_piecewise_left f g x hxmemA
+
+      · apply (Func.ext (Func.comp h iB) g).mp
+        intro x hxmemB
+
+        have hxmemAfalse : St.mem x A → False := by
+          intro hxmemA
+          apply (St.mem_empty x).mp
+          rw [St.mem_congr_right (St.eq_symm hAinterBempty)]
+          apply (St.mem_inter A B x).mpr
+          constructor
+          · exact hxmemA
+          · exact hxmemB
+
+        calc
+          Func.app (Func.comp h iB) x
+
+              =st Func.app h (Func.app iB x)
+                  := Func.app_comp iB h hxmemB
+
+          _   =st Func.app h x
+                  := Func.app_congr_right (
+                      Func.app_incl hBsubAB x hxmemB)
+
+          _   =st Func.app g x
+                  := Func.app_piecewise_right f g x hxmemB hxmemAfalse
+
+
+    exists h
+
+
+    constructor
+    · exact hpiecewise_compsh
+
+    · intro h' hpiecewise_compsh'
+
+      rcases hpiecewise_compsh with ⟨hhiAeqf, hhiBeqg⟩
+      rcases hpiecewise_compsh' with ⟨hh'iAeqf, hh'iBeqg⟩
+
+      apply (Func.ext h' h).mp
+      intro x hxmemAuniB
+
+      have hxmemAorB : St.mem x A ∨ St.mem x B :=
+        (St.mem_uni A B x).mp hxmemAuniB
+
+      rcases hxmemAorB with hxmemA | hxmemB
+      · calc
+        Func.app h' x
+            =st Func.app h' (Func.app iA x)
+                := Func.app_congr_right (
+                    St.eq_symm (Func.app_incl hAsubAB x hxmemA))
+
+        _   =st Func.app (Func.comp h' iA) x
+                := St.eq_symm (Func.app_comp iA h' hxmemA)
+
+        _   =st Func.app f x
+                := Func.app_congr_left hh'iAeqf
+
+        _   =st Func.app (Func.comp h iA) x
+                := Func.app_congr_left (Func.eq_symm hhiAeqf)
+
+        _   =st Func.app h (Func.app iA x)
+                := Func.app_comp iA h hxmemA
+
+        _   =st Func.app h x
+                := Func.app_congr_right (
+                    Func.app_incl hAsubAB x hxmemA)
+
+      · calc
+        Func.app h' x
+            =st Func.app h' (Func.app iB x)
+                := Func.app_congr_right (
+                    St.eq_symm (Func.app_incl hBsubAB x hxmemB))
+
+        _   =st Func.app (Func.comp h' iB) x
+                := St.eq_symm (Func.app_comp iB h' hxmemB)
+
+        _   =st Func.app g x
+                := Func.app_congr_left hh'iBeqg
+
+        _   =st Func.app (Func.comp h iB) x
+                := Func.app_congr_left (Func.eq_symm hhiBeqg)
+
+        _   =st Func.app h (Func.app iB x)
+                := Func.app_comp iB h hxmemB
+
+        _   =st Func.app h x
+                := Func.app_congr_right (
+                    Func.app_incl hBsubAB x hxmemB)
+
+
+
+
+
+
+
+
+
+
+
+
+
+
+
+
+
+
+
+
+
+
+
+
+
