St/Composition.lean
@@ -1,0 +1,1116 @@
+import St.Axioms
+
+
+/- Func definition -/
+
+
+axiom Func : St → St → Type
+axiom Func.eq {A B : St} : Func A B → Func A B → Prop
+infix:50 " =func " => Func.eq
+
+axiom Func.app {A B : St} : Func A B → St → St
+
+axiom Func.tot {A B : St} (f : Func A B) :
+
+    ∀ x : St, St.mem x A → ∃ y : St, St.mem y B ∧ (y =st Func.app f x)
+
+axiom Func.from_Rel {A B : St} {P : St → St → Prop}
+  (h_tot : ∀ x : St, St.mem x A → ∃ y, St.mem y B ∧ P x y)
+  (h_uniq : ∀ x y1 y2 : St, St.mem x A → P x y1 → P x y2 → (y1 =st y2))
+  : Func A B
+
+axiom Func.app_congr_right {A B : St} {f : Func A B} {x y : St} :
+    (x =st y) → (Func.app f x =st Func.app f y)
+
+axiom Func.app_congr_left {A B : St} {f g : Func A B} {x : St} :
+    (f =func g) → (Func.app f x =st Func.app g x)
+
+
+/- Function creation -/
+
+
+axiom Func.exists_const {B : St} (A b : St) (h : St.mem b B) :
+  ∃ f : Func A B, ∀ x, St.mem x A → Func.app f x =st b
+
+axiom Func.exists_incl {A B : St} (hAsubB : St.subset A B) :
+  ∃ f : Func A B, ∀ x, St.mem x A → Func.app f x =st x
+
+axiom Func.exists_piecewise {A B C : St}
+    (f : Func A C) (g : Func B C) :
+
+  ∃ h : Func (St.uni A B) C,
+    (∀ x, St.mem x A → Func.app h x =st Func.app f x) ∧
+    (∀ x, St.mem x B → ¬(St.mem x A) → Func.app h x =st Func.app g x)
+
+axiom Func.exists_congr_dom {A A' B : St}
+    (hAeqA' : A =st A') (f : Func A B) :
+
+  ∃ f' : Func A' B, ∀ x, St.mem x A' → Func.app f' x =st Func.app f x
+
+
+noncomputable def Func.const {B : St} (A b : St)
+    (hbmemB : St.mem b B) : Func A B :=
+
+  Classical.choose (Func.exists_const A b hbmemB)
+
+noncomputable def Func.incl (A B : St)
+    (hAsubB: St.subset A B) : Func A B :=
+
+  Classical.choose (Func.exists_incl hAsubB)
+
+noncomputable def Func.id (A : St) : Func A A :=
+
+  Classical.choose (Func.exists_incl (St.subset_rfl A))
+
+noncomputable def Func.piecewise {A B C : St}
+    (f : Func A C) (g : Func B C) : Func (St.uni A B) C :=
+
+  Classical.choose (Func.exists_piecewise f g)
+
+noncomputable def Func.congr_dom {A A' B : St}
+    (hAeqA' : A =st A') (f : Func A B) : Func A' B :=
+
+  Classical.choose (Func.exists_congr_dom hAeqA' f)
+
+
+theorem Func.app_const {B : St} (A b : St)
+  (hbmemB : St.mem b B) :
+
+  ∀ x, St.mem x A → Func.app (Func.const A b hbmemB) x =st b :=
+
+  Classical.choose_spec (Func.exists_const A b hbmemB)
+
+
+theorem Func.app_incl {A B : St} (hAsubB : St.subset A B) :
+  ∀ x, St.mem x A → Func.app (Func.incl A B hAsubB) x =st x :=
+
+  Classical.choose_spec (Func.exists_incl hAsubB)
+
+
+theorem Func.app_id {A : St} :
+  ∀ x, St.mem x A → Func.app (Func.id A) x =st x :=
+
+  Classical.choose_spec (Func.exists_incl (St.subset_rfl A))
+
+
+theorem Func.app_piecewise_left {A B C : St}
+    (f : Func A C) (g : Func B C) :
+
+  ∀ x, St.mem x A → Func.app (Func.piecewise f g) x =st Func.app f x :=
+
+  (Classical.choose_spec (Func.exists_piecewise f g)).1
+
+
+theorem Func.app_piecewise_right {A B C : St}
+    (f : Func A C) (g : Func B C) :
+
+  ∀ x, St.mem x B → ¬(St.mem x A) →
+    Func.app (Func.piecewise f g) x =st Func.app g x :=
+
+  (Classical.choose_spec (Func.exists_piecewise f g)).2
+
+
+theorem Func.app_congr_dom {A : St}
+    (hAeqA' : A =st A') (f : Func A B) :
+
+  ∀ x, St.mem x A' → Func.app (Func.congr_dom hAeqA' f) x =st
+    Func.app f x :=
+
+  Classical.choose_spec (Func.exists_congr_dom hAeqA' f)
+
+
+/- Equality -/
+
+
+axiom Func.ext {A B : St} (f g : Func A B) :
+    (∀ x : St, St.mem x A → (Func.app f x =st Func.app g x)) ↔
+    f =func g
+
+@[refl]
+theorem Func.eq_rfl {A B : St} (f : Func A B) : f =func f := by
+    apply (Func.ext f f).mp
+    intro x hxmemA
+    rfl
+
+theorem Func.eq_symm {A B : St} {f g : Func A B} :
+    f =func g → g =func f := by
+
+    intro hfeqg
+
+    have hxfxeqgx := (Func.ext f g).mpr hfeqg
+
+    apply (Func.ext g f).mp
+
+    intro x hxmemA
+
+    apply St.eq_symm (hxfxeqgx x hxmemA)
+
+theorem Func.eq_trans {A B : St} {f g h : Func A B} :
+    f =func g → g =func h → f =func h := by
+
+    intro hfeqg hgeqh
+    have hxfxeqgx := (Func.ext f g).mpr hfeqg
+    have hxgxeqhx := (Func.ext g h).mpr hgeqh
+
+    apply (Func.ext f h).mp
+
+    intro x hxmemA
+
+    apply St.eq_trans (hxfxeqgx x hxmemA) (hxgxeqhx x hxmemA)
+
+
+/- Composition -/
+
+
+axiom Func.comp {A B C : St} : (Func B C) → (Func A B) → (Func A C)
+
+axiom Func.app_comp {A B C x : St} (f : Func A B) (g : Func B C) :
+    St.mem x A →
+        (Func.app (Func.comp g f) x =st Func.app g (Func.app f x))
+
+theorem Func.comp_exists {A B C : St} (f : Func A B) (g : Func B C) :
+    ∃ h : Func A C, h =func Func.comp g f := by
+
+    exists (Func.comp g f)
+
+theorem Func.comp_ass {A B C D : St}
+    (f : Func A B) (g : Func B C) (h : Func C D) :
+
+    Func.comp h (Func.comp g f) =func Func.comp (Func.comp h g) f := by
+
+    apply (Func.ext (Func.comp h (Func.comp g f))
+        (Func.comp (Func.comp h g) f)).mp
+
+    intro x hxmemA
+
+    have ⟨y, hymemB, hyeqfx⟩ := Func.tot f x hxmemA
+
+    calc
+        Func.app (Func.comp h (Func.comp g f)) x
+            =st  Func.app h (Func.app (Func.comp g f) x)
+                := Func.app_comp (Func.comp g f) h hxmemA
+
+        _   =st Func.app h (Func.app g (Func.app f x))
+                := Func.app_congr_right (
+                    Func.app_comp f g hxmemA)
+
+        _   =st Func.app h (Func.app g y)
+                := Func.app_congr_right (
+                    Func.app_congr_right (St.eq_symm hyeqfx))
+
+        _   =st Func.app (Func.comp h g) y
+                := St.eq_symm (Func.app_comp g h hymemB)
+
+        _   =st Func.app (Func.comp h g) (Func.app f x)
+                := Func.app_congr_right hyeqfx
+
+        _   =st Func.app (Func.comp (Func.comp h g) f) x
+                := St.eq_symm (
+                    Func.app_comp f (Func.comp h g) hxmemA)
+
+
+theorem Func.comp_congr_left {A B C : St}
+    {f : Func A B} {g1 g2 : Func B C} :
+
+    (g1 =func g2) → (Func.comp g1 f =func Func.comp g2 f) := by
+
+    intro hg1eqg2
+
+    apply (Func.ext (Func.comp g1 f) (Func.comp g2 f)).mp
+
+    intro x hxmemA
+
+    calc
+        (Func.app (Func.comp g1 f) x)
+            =st (Func.app g1 (Func.app f x))
+                := (Func.app_comp f g1 hxmemA)
+
+        _   =st Func.app g2 (Func.app f x)
+                := Func.app_congr_left hg1eqg2
+
+        _   =st Func.app (Func.comp g2 f) x
+                := St.eq_symm (Func.app_comp f g2 hxmemA)
+
+
+theorem Func.comp_congr_right {A B C : St}
+    {f1 f2 : Func A B} {g : Func B C} :
+
+    (f1 =func f2) → (Func.comp g f1 =func Func.comp g f2) := by
+
+    intro hf1eqf2
+
+    apply (Func.ext (Func.comp g f1) (Func.comp g f2)).mp
+
+    intro x hxmemA
+
+    calc
+        (Func.app (Func.comp g f1) x)
+            =st (Func.app g (Func.app f1 x))
+                := (Func.app_comp f1 g hxmemA)
+
+        _   =st Func.app g (Func.app f2 x)
+                := Func.app_congr_right (
+                    Func.app_congr_left hf1eqf2)
+
+        _   =st Func.app (Func.comp g f2) x
+                := St.eq_symm (Func.app_comp f2 g hxmemA)
+
+
+/- Injection & Onto -/
+
+
+axiom Func.inj {A B : St} (f : Func A B) : Prop
+
+axiom Func.is_inj {A B : St} (f : Func A B) :
+    Func.inj f ↔
+
+    ∀ x x' : St, St.mem x A → St.mem x' A →
+        (Func.app f x =st Func.app f x') → x =st x'
+
+
+theorem Func.comp_inj {A B C : St} (f : Func A B) (g : Func B C) :
+    Func.inj f → Func.inj g → Func.inj (Func.comp g f) := by
+
+    intro hinjf hinjg
+
+    replace hinjf := (Func.is_inj f).mp hinjf
+    replace hinjg := (Func.is_inj g).mp hinjg
+
+    apply (Func.is_inj (Func.comp g f)).mpr
+
+    intro x x' hxmemA hx'memA hgfxeqgfx'
+
+    have ⟨y, hymemB, hyeqfx⟩ := Func.tot f x hxmemA
+    have ⟨y', hy'memB, hy'eqfx'⟩ := Func.tot f x' hx'memA
+
+    have hgyeqgy' : Func.app g y =st Func.app g y' := by
+        calc
+            Func.app g y
+                =st Func.app g (Func.app f x)
+                    := Func.app_congr_right hyeqfx
+            _   =st Func.app (Func.comp g f) x
+                    := St.eq_symm (Func.app_comp f g hxmemA)
+            _   =st Func.app (Func.comp g f) x'
+                    := hgfxeqgfx'
+            _   =st Func.app g (Func.app f x')
+                    := Func.app_comp f g hx'memA
+            _   =st Func.app g y'
+                    := Func.app_congr_right (St.eq_symm hy'eqfx')
+
+    have hyeqy' := hinjg y y' hymemB hy'memB hgyeqgy'
+
+    have hfxeqfx' : Func.app f x =st Func.app f x' := by
+        calc
+            Func.app f x
+                =st y
+                    := St.eq_symm hyeqfx
+            _   =st y'
+                    := hyeqy'
+            _   =st Func.app f x'
+                    := hy'eqfx'
+
+    have hxeqx' := hinjf x x' hxmemA hx'memA hfxeqfx'
+
+    exact hxeqx'
+
+
+axiom Func.onto {A B : St} (f : Func A B) : Prop
+
+axiom Func.is_onto {A B : St} (f : Func A B) :
+    Func.onto f ↔
+
+    ∀ y : St, St.mem y B → ∃ x : St, St.mem x A ∧ (y =st Func.app f x)
+
+theorem Func.comp_onto {A B C : St} (f : Func A B) (g : Func B C) :
+    Func.onto f → Func.onto g → Func.onto (Func.comp g f) := by
+
+    intro hontof hontog
+
+    replace hontof := (Func.is_onto f).mp hontof
+    replace hontog := (Func.is_onto g).mp hontog
+
+    apply (Func.is_onto (Func.comp g f)).mpr
+
+    intro z hzmemC
+
+    rcases (hontog z hzmemC) with ⟨y, hymemB, hzeqgy⟩
+    rcases (hontof y hymemB) with ⟨x, hxmemA, hyeqfx⟩
+
+    exists x
+    constructor
+    · exact hxmemA
+    · calc
+        z
+            =st Func.app g y
+                := hzeqgy
+
+        _   =st Func.app g (Func.app f x)
+                := Func.app_congr_right hyeqfx
+
+        _   =st Func.app (Func.comp g f) x
+                := St.eq_symm (Func.app_comp f g hxmemA)
+
+
+theorem Func.empty_inj {A : St} (f : Func St.empty A) :
+    Func.inj f := by
+
+    apply (Func.is_inj f).mpr
+    intro x x' hxmemEmp hx'memEmp
+
+    exfalso
+    apply (St.mem_empty x).mp
+    exact hxmemEmp
+
+
+theorem Func.canc_comp_left {A B C : St}
+    (f f' : Func A B) (g : Func B C) :
+
+    Func.comp g f =func Func.comp g f' → Func.inj g → f =func f' := by
+
+    intro hgfeqgf' hinjg
+
+    apply (Func.ext f f').mp
+
+    intro x hxmemA
+
+    have hgfxeqgf'x :=
+        (Func.ext (Func.comp g f) (Func.comp g f')).mpr hgfeqgf'
+
+    replace hgfxeqgf'x := hgfxeqgf'x x hxmemA
+
+    replace hinjg := (Func.is_inj g).mp hinjg
+
+    have ⟨y, hymemB, hyeqfx⟩ := Func.tot f x hxmemA
+    have ⟨y', hy'memB, hy'eqf'x⟩ := Func.tot f' x hxmemA
+
+    have hgyeqgy' : Func.app g y =st Func.app g y' := by
+        calc
+            Func.app g y
+                =st Func.app g (Func.app f x)
+                    := Func.app_congr_right hyeqfx
+
+            _   =st Func.app (Func.comp g f) x
+                    := St.eq_symm (Func.app_comp f g hxmemA)
+
+            _   =st Func.app (Func.comp g f') x
+                    := hgfxeqgf'x
+
+            _   =st Func.app g (Func.app f' x)
+                    := Func.app_comp f' g hxmemA
+
+            _   =st Func.app g y'
+                    := St.eq_symm (Func.app_congr_right hy'eqf'x)
+
+
+    have hyeqy' := hinjg y y' hymemB hy'memB hgyeqgy'
+
+    have hfxeqf'x : Func.app f x =st Func.app f' x := by
+        calc
+            Func.app f x
+            _   =st y
+                := St.eq_symm hyeqfx
+
+            _   =st y'
+                := hyeqy'
+
+            _   =st Func.app f' x
+                := hy'eqf'x
+
+    exact hfxeqf'x
+
+--   ∀ x x' : St, St.mem x A → St.mem x' A →
+--      (Func.app f x =st Func.app f x') → x =st x'
+
+theorem Func.no_canc_comp_left :
+
+    ∃ A B C : St, ∃ f f' : Func A B, ∃ g : Func B C,
+
+        (f =func f' → False) ∧
+        (Func.comp g f =func Func.comp g f') := by
+
+    let A := (St.pair St.empty (St.singlet St.empty))
+    let B := A
+    let C := B
+
+    exists A, B, C
+
+    have hzeromemA : St.mem St.empty A := by
+        apply (St.mem_pair St.empty (St.singlet St.empty) St.empty).mpr
+        left
+        rfl
+
+    have honememA : St.mem (St.singlet St.empty) A := by
+        apply (St.mem_pair St.empty (St.singlet St.empty)
+            (St.singlet St.empty)).mpr
+        right
+        rfl
+
+    have hzeromemB := hzeromemA
+    have honememB := honememA
+    have hzeromemC := hzeromemB
+
+    let f : Func A B := Func.const A St.empty hzeromemB
+    let f' : Func A B := Func.const A (St.singlet St.empty) honememB
+
+    exists f, f'
+
+
+    let g : Func B C := Func.const B St.empty hzeromemC
+
+    exists g
+
+    constructor
+    ·   intro hfeqf'
+        have hzeroeqone : St.empty =st St.singlet St.empty := by
+            --intro x hxmemA
+            calc
+                St.empty
+                    =st Func.app f St.empty
+                        := St.eq_symm (Func.app_const A
+                            St.empty hzeromemB
+                            St.empty hzeromemA)
+
+                _   =st Func.app f' St.empty
+                        := (Func.ext f f').mpr hfeqf' St.empty hzeromemA
+
+                _   =st St.singlet St.empty
+                        := Func.app_const A
+                            (St.singlet St.empty) honememB
+                            St.empty hzeromemA 
+
+        have hzeromemzero : St.mem St.empty St.empty := by
+            rw [(St.mem_congr_right hzeroeqone)]
+            apply (St.mem_singlet St.empty St.empty).mpr
+            rfl
+
+        apply (St.mem_empty St.empty).mp hzeromemzero
+
+    ·
+        apply (Func.ext (Func.comp g f) (Func.comp g f')).mp
+
+        intro x hxmemA
+
+        have hxeqzeroorxeqone :
+            (x =st St.empty) ∨ (x =st (St.singlet St.empty)) := by
+
+            apply (St.mem_pair St.empty
+                (St.singlet St.empty) x).mp hxmemA
+
+        rcases hxeqzeroorxeqone with hxeqzero | hxeqone
+        · -- app (comp g f) x = app (comp g f') x
+          calc
+            Func.app (Func.comp g f) x
+                =st Func.app (Func.comp g f) St.empty
+                    := Func.app_congr_right hxeqzero
+
+            _   =st Func.app g (Func.app f St.empty)
+                    := Func.app_comp f g hzeromemA
+
+            _   =st Func.app g St.empty
+                    := Func.app_congr_right (
+                        Func.app_const A
+                            St.empty hzeromemB St.empty hzeromemA)
+
+            _   =st St.empty
+                    := Func.app_const B
+                        St.empty hzeromemC St.empty hzeromemB
+
+            _   =st Func.app g (St.singlet St.empty)
+                    := St.eq_symm (Func.app_const B
+                        St.empty hzeromemC
+                        (St.singlet St.empty) honememB)
+
+            _   =st Func.app g (Func.app f' St.empty)
+                    := Func.app_congr_right (St.eq_symm (
+                        Func.app_const A
+                            (St.singlet St.empty) honememB
+                            St.empty hzeromemA))
+
+            _   =st Func.app (Func.comp g f') St.empty
+                    := St.eq_symm (Func.app_comp f' g hzeromemA)
+
+            _   =st Func.app (Func.comp g f') x
+                    := Func.app_congr_right (St.eq_symm hxeqzero)
+
+        · -- app (comp g f) zero = app (comp g f') zero
+          calc
+            Func.app (Func.comp g f) x
+                =st Func.app (Func.comp g f) (St.singlet St.empty)
+                    := Func.app_congr_right hxeqone
+
+            _   =st Func.app g (Func.app f (St.singlet St.empty))
+                    := Func.app_comp f g honememA
+
+            _   =st Func.app g St.empty
+                    := Func.app_congr_right (
+                        Func.app_const A
+                            St.empty hzeromemB
+                            (St.singlet St.empty) honememA)
+
+            _   =st St.empty
+                    := Func.app_const B
+                        St.empty hzeromemC St.empty hzeromemB
+
+            _   =st Func.app g (St.singlet St.empty)
+                    := St.eq_symm (Func.app_const B
+                        St.empty hzeromemC
+                        (St.singlet St.empty) honememB)
+
+            _   =st Func.app g (Func.app f' (St.singlet St.empty))
+                    := Func.app_congr_right (St.eq_symm (
+                        Func.app_const A
+                            (St.singlet St.empty) honememB
+                            (St.singlet St.empty) honememA))
+
+            _   =st Func.app (Func.comp g f') (St.singlet St.empty)
+                    := St.eq_symm (Func.app_comp f' g honememA)
+
+            _   =st Func.app (Func.comp g f') x
+                    := Func.app_congr_right (St.eq_symm hxeqone)
+
+
+theorem Func.canc_comp_right {A B C : St}
+    (f : Func A B) (g g' : Func B C) :
+
+    Func.comp g f =func Func.comp g' f → Func.onto f → g =func g' := by
+
+    intro hgfeqg'f hontof
+
+    apply (Func.ext g g').mp
+
+    intro y hymemB
+
+    replace hontof := (Func.is_onto f).mp hontof
+    replace hontof := hontof y hymemB
+
+    have ⟨x, hxmemA, hyeqfx⟩ := hontof
+
+    have hgfxeqg'fx :=
+        (Func.ext (Func.comp g f) (Func.comp g' f)).mpr hgfeqg'f
+
+    replace hgfxeqg'fx := hgfxeqg'fx x hxmemA
+
+    have ⟨z, hzmemC, hzeqgy⟩ := Func.tot g y hymemB
+    have ⟨z', hz'memC, hz'eqg'y⟩ := Func.tot g' y hymemB
+
+    have hgyeqg'y : Func.app g y =st Func.app g' y := by
+        calc
+            Func.app g y
+                =st Func.app g (Func.app f x)
+                    := Func.app_congr_right hyeqfx
+
+            _   =st Func.app (Func.comp g f) x
+                    := St.eq_symm (Func.app_comp f g hxmemA)
+
+            _   =st Func.app (Func.comp g' f) x
+                    := hgfxeqg'fx
+
+            _   =st Func.app g' (Func.app f x)
+                    := Func.app_comp f g' hxmemA
+
+            _   =st Func.app g' y
+                    := St.eq_symm (Func.app_congr_right hyeqfx)
+
+    exact hgyeqg'y
+
+theorem Func.no_canc_comp_right :
+
+    ∃ A B C : St, ∃ f : Func A B, ∃ g g' : Func B C,
+
+        (g =func g' → False) ∧
+        (Func.comp g f =func Func.comp g' f) := by
+
+    let A := (St.pair St.empty (St.singlet St.empty))
+    let B := A
+    let C := B
+    let B1 := St.singlet St.empty
+    let B2 := St.singlet (St.singlet St.empty)
+
+    have hb1b2eqb : St.uni B1 B2 =st B := by
+        apply (St.ext (St.uni B1 B2) B).mp
+        intro x
+        constructor
+        · intro hxmemB1B2
+          have hxmemB1orxmemB2 := (St.mem_uni B1 B2 x).mp hxmemB1B2
+          rcases hxmemB1orxmemB2 with hxmemB1 | hxmemB2
+          · have hxeqempty := (St.mem_singlet St.empty x).mp hxmemB1
+            apply (St.mem_pair St.empty (St.singlet St.empty) x).mpr
+            left
+            exact hxeqempty
+          · have hxeqone :=
+                (St.mem_singlet (St.singlet St.empty) x).mp hxmemB2
+            apply (St.mem_pair St.empty (St.singlet St.empty) x).mpr
+            right
+            exact hxeqone
+        · intro hxmemB
+          have hxeqzeroorxeqone :=
+            (St.mem_pair St.empty (St.singlet St.empty) x).mp hxmemB
+
+          apply (St.mem_uni B1 B2 x).mpr
+          rcases hxeqzeroorxeqone with hxeqzero | hxeqone
+          · left
+            apply (St.mem_singlet St.empty x).mpr
+            exact hxeqzero
+          · right
+            apply (St.mem_singlet (St.singlet St.empty) x).mpr
+            exact hxeqone
+
+
+    exists A, B, C
+
+    have hzeromemB1 : St.mem St.empty B1 := by
+        apply (St.mem_singlet St.empty St.empty).mpr
+        rfl
+
+    have honememB1false : St.mem (St.singlet St.empty) B1 → False := by
+        intro honememB1
+        have honeeqzero : St.singlet St.empty =st St.empty :=
+            (St.mem_singlet St.empty (St.singlet St.empty)).mp honememB1
+
+        have hzeromemzero : St.mem St.empty St.empty := by
+            rw [St.mem_congr_right (St.eq_symm honeeqzero)]
+            apply (St.mem_singlet St.empty St.empty).mpr
+            rfl
+
+        apply (St.mem_empty St.empty).mp hzeromemzero
+
+    have honememB2 : St.mem (St.singlet St.empty) B2 := by
+        apply (St.mem_singlet
+            (St.singlet St.empty) (St.singlet St.empty)).mpr
+        rfl
+
+    have hzeromemA : St.mem St.empty A := by
+        apply (St.mem_pair St.empty (St.singlet St.empty) St.empty).mpr
+        left
+        rfl
+
+    have honememA : St.mem (St.singlet St.empty) A := by
+        apply (St.mem_pair St.empty (St.singlet St.empty)
+            (St.singlet St.empty)).mpr
+        right
+        rfl
+
+    have hzeromemB := hzeromemA
+    have honememB := honememA
+    have hzeromemC := hzeromemB
+    have honememC := honememB
+
+    let f : Func A B := Func.const A St.empty hzeromemB
+
+    exists f
+
+
+    let g : Func B C := Func.const B St.empty hzeromemC
+    let h1 : Func B1 C := Func.const B1 St.empty hzeromemC
+    let h2 : Func B2 C := Func.const B2 (St.singlet St.empty) honememC
+    let h : Func (St.uni B1 B2) C := Func.piecewise h1 h2
+    let g' : Func B C := Func.congr_dom hb1b2eqb h
+
+    exists g, g'
+
+
+    constructor
+    ·   intro hgeqg'
+        have hzeroeqone : St.empty =st St.singlet St.empty := by
+            calc
+                St.empty
+                    =st Func.app g (St.singlet St.empty)
+                        := St.eq_symm (Func.app_const B
+                            St.empty hzeromemC
+                            (St.singlet St.empty) honememB)
+
+                _   =st Func.app g' (St.singlet St.empty)
+                        := (Func.ext g g').mpr hgeqg'
+                            (St.singlet St.empty) honememB
+
+                _   =st Func.app h (St.singlet St.empty)
+                        := Func.app_congr_dom
+                            hb1b2eqb h
+
+                            (St.singlet St.empty) honememB
+
+
+                _   =st Func.app h2 (St.singlet St.empty)
+                        := Func.app_piecewise_right h1 h2
+
+                            (St.singlet St.empty) honememB2
+                            honememB1false
+
+                _   =st St.singlet St.empty
+                        := Func.app_const B2
+                            (St.singlet St.empty) honememC
+                            (St.singlet St.empty) honememB2
+
+        have hzeromemzero : St.mem St.empty St.empty := by
+            rw [(St.mem_congr_right hzeroeqone)]
+            apply (St.mem_singlet St.empty St.empty).mpr
+            rfl
+
+        apply (St.mem_empty St.empty).mp hzeromemzero
+
+    ·
+        apply (Func.ext (Func.comp g f) (Func.comp g' f)).mp
+
+        intro x hxmemA
+
+        have hxeqzeroorxeqone :
+            (x =st St.empty) ∨ (x =st (St.singlet St.empty)) := by
+
+            apply (St.mem_pair St.empty
+                (St.singlet St.empty) x).mp hxmemA
+
+        rcases hxeqzeroorxeqone with hxeqzero | hxeqone
+        · -- app (comp g f) x = app (comp g' f) x
+          calc
+            Func.app (Func.comp g f) x
+                =st Func.app (Func.comp g f) St.empty
+                    := Func.app_congr_right hxeqzero
+
+            _   =st Func.app g (Func.app f St.empty)
+                    := Func.app_comp f g hzeromemA
+
+            _   =st Func.app g St.empty
+                    := Func.app_congr_right (
+                        Func.app_const A
+                            St.empty hzeromemB St.empty hzeromemA)
+
+            _   =st St.empty
+                    := Func.app_const B
+                        St.empty hzeromemC St.empty hzeromemB
+
+            _   =st Func.app h1 St.empty
+                    := St.eq_symm (Func.app_const B1
+                        St.empty hzeromemC
+                        St.empty hzeromemB1)
+
+            _   =st Func.app h St.empty
+                    := St.eq_symm (
+                        Func.app_piecewise_left h1 h2
+                            St.empty hzeromemB1)
+
+            _   =st Func.app g' St.empty
+                    := St.eq_symm (Func.app_congr_dom hb1b2eqb h
+                        St.empty hzeromemB)
+
+            --_   =st Func.app (Func.comp g' f) St.empty
+
+            _   =st Func.app g' (Func.app f St.empty)
+                    := Func.app_congr_right (St.eq_symm (
+                        Func.app_const A
+                            St.empty hzeromemB
+                            St.empty hzeromemA))
+
+            _   =st Func.app (Func.comp g' f) St.empty
+                    := St.eq_symm (Func.app_comp f g' hzeromemA)
+
+            _   =st Func.app (Func.comp g' f) x
+                    := Func.app_congr_right (St.eq_symm hxeqzero)
+
+        · -- app (comp g f) one = app (comp g' f) one
+          calc
+            Func.app (Func.comp g f) x
+                =st Func.app (Func.comp g f) (St.singlet St.empty)
+                    := Func.app_congr_right hxeqone
+
+            _   =st Func.app g (Func.app f (St.singlet St.empty))
+                    := Func.app_comp f g honememA
+
+            _   =st Func.app g St.empty
+                    := Func.app_congr_right (
+                        Func.app_const A
+                            St.empty hzeromemB
+                            (St.singlet St.empty) honememA)
+
+            _   =st St.empty
+                    := Func.app_const B
+                        St.empty hzeromemC St.empty hzeromemB
+
+            _   =st Func.app h1 St.empty
+                    := St.eq_symm (Func.app_const B1
+                        St.empty hzeromemC
+                        St.empty hzeromemB1)
+
+            _   =st Func.app h St.empty
+                    := St.eq_symm (
+                        Func.app_piecewise_left h1 h2
+                            St.empty hzeromemB1)
+
+            _   =st Func.app g' St.empty
+                    := St.eq_symm (Func.app_congr_dom hb1b2eqb h
+                        St.empty hzeromemB)
+
+            _   =st Func.app g' (Func.app f (St.singlet St.empty))
+                    := Func.app_congr_right (St.eq_symm (
+                        Func.app_const A
+                            St.empty hzeromemB
+                            (St.singlet St.empty) honememA))
+
+            _   =st Func.app (Func.comp g' f) (St.singlet St.empty)
+                    := St.eq_symm (Func.app_comp f g' honememA)
+
+            _   =st Func.app (Func.comp g' f) x
+                    := Func.app_congr_right (St.eq_symm hxeqone)
+
+
+
+theorem comp_inj_then_f_inj
+    (hgfinj : Func.inj (Func.comp g f)) :
+
+    Func.inj f := by
+
+    apply (Func.is_inj f).mpr
+
+    intro x x' hxmemA hx'memA hfxeqfx'
+
+    have hgfxeqgfx' :
+        Func.app (Func.comp g f) x =st Func.app (Func.comp g f) x' := by
+
+        calc
+            Func.app (Func.comp g f) x
+                =st Func.app g (Func.app f x)
+                    := Func.app_comp f g hxmemA 
+
+            _   =st Func.app g (Func.app f x')
+                    := Func.app_congr_right hfxeqfx'
+
+            _   =st Func.app (Func.comp g f) x'
+                    := St.eq_symm (Func.app_comp f g hx'memA)
+
+    apply (Func.is_inj (Func.comp g f)).mp hgfinj
+        x x' hxmemA hx'memA hgfxeqgfx'
+
+
+theorem Func.comp_inj_no_g_inj :
+
+    ∃ A B C : St, ∃ f : Func A B, ∃ g : Func B C,
+
+        Func.inj (Func.comp g f) ∧ (Func.inj g → False) := by
+
+    let A := St.singlet St.empty
+    let B := St.pair St.empty (St.singlet St.empty)
+    let C := A
+
+    have hzeromemA : St.mem St.empty A := by
+        apply (St.mem_singlet St.empty St.empty).mpr
+        rfl
+
+    have hzeromemB : St.mem St.empty B := by
+        apply (St.mem_pair St.empty (St.singlet St.empty) St.empty).mpr
+        left
+        rfl
+
+    have honememB : St.mem (St.singlet St.empty) B := by
+        apply (St.mem_pair St.empty (St.singlet St.empty)
+            (St.singlet St.empty)).mpr
+        right
+        rfl
+
+    have hzeromemC := hzeromemA
+
+    let f := Func.const A St.empty hzeromemB
+    let g := Func.const B St.empty hzeromemC
+
+
+    exists A, B, C, f, g
+
+    constructor
+    · apply (Func.is_inj (Func.comp g f)).mpr
+      intro x x' hxmemA hx'memA hgfxeqgfx'
+
+      have hx'eqzero : x' =st St.empty := by
+        apply (St.mem_singlet St.empty x').mp hx'memA
+
+      have hxeqzero : x =st St.empty := by
+        apply (St.mem_singlet St.empty x).mp hxmemA
+
+      calc
+        x =st St.empty := hxeqzero
+        _ =st x' := St.eq_symm hx'eqzero
+
+    · intro hginj
+      have hzeroeqone : St.empty =st St.singlet St.empty := by
+
+        apply (Func.is_inj g).mp hginj St.empty (St.singlet St.empty)
+            hzeromemB honememB
+
+        calc
+            Func.app g St.empty
+                =st St.empty
+                    := Func.app_const B
+                        St.empty hzeromemC
+                        St.empty hzeromemB
+
+            _   =st Func.app g (St.singlet St.empty)
+                    := St.eq_symm (
+                        Func.app_const B
+                            St.empty hzeromemC
+                            (St.singlet St.empty) honememB)
+
+      have hzeromemzero : St.mem St.empty St.empty := by
+        rw [St.mem_congr_right hzeroeqone]
+        apply (St.mem_singlet St.empty St.empty).mpr
+        rfl
+
+      apply (St.mem_empty St.empty).mp hzeromemzero
+
+theorem comp_onto_then_g_onto
+    (hgfonto : Func.onto (Func.comp g f)) :
+
+    Func.onto g := by
+
+    apply (Func.is_onto g).mpr
+
+    intro z hzmemC
+
+    replace hgfonto := (Func.is_onto (Func.comp g f)).mp hgfonto
+    rcases (hgfonto z hzmemC) with ⟨x, hxmemA, hzeqgfx⟩
+    have ⟨y, hymemB, hyeqfx⟩ := Func.tot f x hxmemA
+
+    exists y
+
+    constructor
+    · exact hymemB
+    · calc
+        z =st Func.app (Func.comp g f) x
+            := hzeqgfx
+
+        _ =st Func.app g (Func.app f x)
+            := Func.app_comp f g hxmemA
+
+        _ =st Func.app g y
+            := Func.app_congr_right (St.eq_symm hyeqfx)
+
+theorem Func.comp_onto_no_f_onto :
+
+    ∃ A B C : St, ∃ f : Func A B, ∃ g : Func B C,
+
+        Func.onto (Func.comp g f) ∧ (Func.onto f → False) := by
+
+
+    let A := St.singlet St.empty
+    let B := St.pair St.empty (St.singlet St.empty)
+    let C := A
+
+    have hzeromemA : St.mem St.empty A := by
+        apply (St.mem_singlet St.empty St.empty).mpr
+        rfl
+
+    have hzeromemB : St.mem St.empty B := by
+        apply (St.mem_pair St.empty (St.singlet St.empty) St.empty).mpr
+        left
+        rfl
+
+    have honememB : St.mem (St.singlet St.empty) B := by
+        apply (St.mem_pair St.empty (St.singlet St.empty)
+            (St.singlet St.empty)).mpr
+        right
+        rfl
+
+    have hzeromemC := hzeromemA
+
+    let f := Func.const A St.empty hzeromemB
+    let g := Func.const B St.empty hzeromemC
+
+    exists A, B, C, f, g
+
+    constructor
+    · apply (Func.is_onto (Func.comp g f)).mpr
+      intro z hzmemC
+
+      exists St.empty
+      constructor
+      · exact hzeromemA
+      · have hzeqzero : z =st St.empty := by
+            apply (St.mem_singlet St.empty z).mp hzmemC
+
+        calc
+            z =st St.empty
+                := hzeqzero
+
+            _ =st Func.app g St.empty
+                := St.eq_symm (
+                    Func.app_const B
+                        St.empty hzeromemC
+                        St.empty hzeromemB)
+
+            _ =st Func.app g (Func.app f St.empty)
+                := Func.app_congr_right (
+                    St.eq_symm (
+                        Func.app_const A
+                            St.empty hzeromemB
+                            St.empty hzeromemA))
+
+            _ =st Func.app (Func.comp g f) St.empty
+                := St.eq_symm (
+                    Func.app_comp f g hzeromemA)
+
+
+    · intro hfonto
+
+      replace hfonto := (Func.is_onto f).mp hfonto
+      rcases (hfonto (St.singlet St.empty) honememB)
+        with ⟨x, hxmemA, honeeqfx⟩
+
+      have hxeqzero : x =st St.empty := by
+        apply (St.mem_singlet St.empty x).mp hxmemA
+
+      have hzeroeqone : St.empty =st St.singlet St.empty := by
+        calc
+            St.empty
+                =st Func.app f St.empty
+                    := St.eq_symm (
+                        Func.app_const A
+                            St.empty hzeromemB
+                            St.empty hzeromemA)
+
+            _   =st Func.app f x
+                    := Func.app_congr_right (St.eq_symm hxeqzero)
+
+            _   =st St.singlet St.empty
+                    := St.eq_symm honeeqfx
+
+      have hzeromemzero : St.mem St.empty St.empty := by
+        rw [St.mem_congr_right hzeroeqone]
+        apply (St.mem_singlet St.empty St.empty).mpr
+        rfl
+
+      apply (St.mem_empty St.empty).mp
+      exact hzeromemzero
+
+
+
+
+/-
+    have hfinj : Func.inj f := by
+        apply (Func.is_inj f).mpr
+        intro x x' hxmemA hx'memA hfxeqfx'
+
+        calc
+            x =st Func.app f x
+                := St.eq_symm (Func.app_id x hxmemA)
+
+            _ =st Func.app f x'
+                := hfxeqfx'
+
+            _ =st x'
+                := Funx.app_id x' hx'memA
+
+
+-/
+
+
+
+
+
+
+
+
+
+
+
+
+
+
+
+
+
