St/Multiplication.lean
@@ -1,0 +1,878 @@
+import St.Order
+
+
+/- Multiplication definition -/
+
+
+axiom Nt.mul : Nt → Nt → Nt
+
+axiom Nt.mul_zero_right (a : Nt) :
+    Nt.mul a Nt.zero =nt Nt.zero
+
+axiom Nt.mul_succ_right (a b : Nt) :
+    Nt.mul a (Nt.succ b) =nt Nt.add a (Nt.mul a b)
+
+
+/- Multiplication properties -/
+
+
+theorem Nt.mul_zero_left (a : Nt) : Nt.mul Nt.zero a =nt Nt.zero := by
+
+    let P (n : Nt) : Prop := Nt.mul Nt.zero n =nt Nt.zero
+
+    have h_base : P Nt.zero := by
+        exact Nt.mul_zero_right Nt.zero
+
+    have h_step : ∀ n : Nt, P n → P (Nt.succ n) := by
+        intro n hPn
+
+        calc
+            (Nt.mul Nt.zero (Nt.succ n))
+                =nt (Nt.add Nt.zero (Nt.mul Nt.zero n))
+                    := Nt.mul_succ_right Nt.zero n
+
+            _   =nt Nt.mul Nt.zero n
+                    := Nt.add_zero_left (Nt.mul Nt.zero n)
+
+            _   =nt Nt.zero
+                    := hPn
+
+    apply Nt.induction P h_base h_step a
+
+
+theorem Nt.mul_succ_left (a b : Nt) :
+    Nt.mul (Nt.succ a) b =nt Nt.add (Nt.mul a b) b := by
+
+    let P (n m : Nt) : Prop :=
+        Nt.mul (Nt.succ n) m =nt Nt.add (Nt.mul n m) m
+
+    have h_base : ∀ (m : Nt), P Nt.zero m := by
+
+        let P_base (m : Nt) : Prop := P Nt.zero m
+
+        have h_base_base : P Nt.zero Nt.zero := by
+
+            calc
+                (Nt.mul (Nt.succ Nt.zero) Nt.zero)
+                    =nt Nt.zero
+                        := Nt.mul_zero_right (Nt.succ Nt.zero)
+                _   =nt Nt.add Nt.zero Nt.zero
+                        := Nt.eq_symm (Nt.add_zero_right Nt.zero)
+
+                _   =nt Nt.add (Nt.mul Nt.zero Nt.zero) Nt.zero
+                        := Nt.add_congr_left
+                            (Nt.eq_symm (Nt.mul_zero_right Nt.zero))
+
+        have h_base_step :
+            ∀ (m : Nt), P Nt.zero m → P Nt.zero (Nt.succ m) := by
+
+            intro m hPm
+
+            calc
+                (Nt.mul (Nt.succ Nt.zero) (Nt.succ m))
+                    =nt (Nt.add (Nt.succ Nt.zero)
+                            (Nt.mul (Nt.succ Nt.zero) m))
+                        := Nt.mul_succ_right (Nt.succ Nt.zero) m
+
+                _   =nt (Nt.add (Nt.succ Nt.zero)
+                            (Nt.add (Nt.mul Nt.zero m) m))
+                        := Nt.add_congr_right hPm
+
+                _   =nt (Nt.succ (Nt.add Nt.zero
+                                (Nt.add (Nt.mul Nt.zero m) m)))
+                        := Nt.add_succ_left Nt.zero
+                            (Nt.add (Nt.mul Nt.zero m) m)
+
+                _   =nt (Nt.add Nt.zero
+                            (Nt.succ (Nt.add (Nt.mul Nt.zero m) m)))
+                        := Nt.eq_symm (Nt.add_succ_right Nt.zero
+                            (Nt.add (Nt.mul Nt.zero m) m))
+
+                _   =nt (Nt.add Nt.zero
+                            (Nt.add (Nt.mul Nt.zero m) (Nt.succ m)))
+                        := Nt.add_congr_right (Nt.eq_symm
+                            (Nt.add_succ_right (Nt.mul Nt.zero m) m))
+
+                _   =nt (Nt.add (Nt.add Nt.zero (Nt.mul Nt.zero m))
+                            (Nt.succ m))
+                        := Nt.add_ass Nt.zero
+                            (Nt.mul Nt.zero m) (Nt.succ m)
+
+                _   =nt (Nt.add (Nt.mul Nt.zero (Nt.succ m))
+                            (Nt.succ m))
+                        := Nt.add_congr_left (Nt.eq_symm
+                            (Nt.mul_succ_right Nt.zero m))
+
+        intro m
+
+        apply Nt.induction P_base h_base_base h_base_step m
+
+
+    have h_step : ∀ (m : Nt), ∀ (n : Nt), P n m → P (Nt.succ n) m := by
+
+        let P_step (m : Nt) : Prop :=
+            ∀ (n : Nt), P n m → P (Nt.succ n) m
+
+        have h_step_base :
+            ∀ (n : Nt), P n Nt.zero → P (Nt.succ n) Nt.zero := by
+
+            intro n hPn
+
+            calc
+                Nt.mul (Nt.succ (Nt.succ n)) Nt.zero
+                    =nt Nt.zero
+                        := Nt.mul_zero_right (Nt.succ (Nt.succ n))
+
+                _   =nt (Nt.mul (Nt.succ n) Nt.zero)
+                        := Nt.eq_symm (Nt.mul_zero_right (Nt.succ n))
+
+                _   =nt Nt.add (Nt.mul (Nt.succ n) Nt.zero) Nt.zero
+                        := Nt.eq_symm (Nt.add_zero_right 
+                            (Nt.mul (Nt.succ n) Nt.zero))
+
+
+        have h_step_step :
+            ∀ (m : Nt),
+                (∀ (n : Nt), P n m → P (Nt.succ n) m)
+                →
+                (∀ (n : Nt),  P n (Nt.succ m) →
+                    P (Nt.succ n) (Nt.succ m))
+            := by
+
+            intro m h_step_n n hPnsuccm
+
+            have hPsuccnm : P (Nt.succ n) m := by
+                apply h_step_n n
+
+                apply Nt.add_canc_left (Nt.succ n)
+
+                calc
+                    (Nt.add (Nt.succ n) (Nt.mul (Nt.succ n) m))
+                        =nt (Nt.mul (Nt.succ n) (Nt.succ m))
+                            := Nt.eq_symm
+                                (Nt.mul_succ_right (Nt.succ n) m)
+
+                    _   =nt (Nt.add (Nt.mul n (Nt.succ m)) (Nt.succ m))
+                            := hPnsuccm
+
+                    _   =nt (Nt.add (Nt.add n (Nt.mul n m)) (Nt.succ m))
+                            := Nt.add_congr_left (Nt.mul_succ_right n m)
+
+                    _   =nt (Nt.add n (Nt.add (Nt.mul n m) (Nt.succ m)))
+                            := Nt.eq_symm
+                                (Nt.add_ass n (Nt.mul n m) (Nt.succ m))
+
+                    _   =nt (Nt.add n (Nt.succ (Nt.add (Nt.mul n m) m)))
+                            := Nt.add_congr_right
+                                (Nt.add_succ_right (Nt.mul n m) m)
+
+                    _   =nt (Nt.succ (Nt.add n (Nt.add (Nt.mul n m) m)))
+                            := (Nt.add_succ_right n
+                                (Nt.add (Nt.mul n m) m))
+
+                    _   =nt (Nt.add (Nt.succ n) (Nt.add (Nt.mul n m) m))
+                            := (Nt.eq_symm (Nt.add_succ_left n
+                                (Nt.add (Nt.mul n m) m)))
+
+
+            calc
+                (Nt.mul (Nt.succ (Nt.succ n)) (Nt.succ m))
+                    =nt (Nt.add (Nt.succ (Nt.succ n))
+                                (Nt.mul (Nt.succ (Nt.succ n)) m))
+                        := Nt.mul_succ_right (Nt.succ (Nt.succ n)) m
+
+                _   =nt (Nt.add (Nt.succ (Nt.succ n))
+                                (Nt.add (Nt.mul (Nt.succ n) m) m))
+                        := Nt.add_congr_right hPsuccnm
+
+                _   =nt (Nt.succ (Nt.add (Nt.succ n)
+                                (Nt.add (Nt.mul (Nt.succ n) m) m)))
+                        := Nt.add_succ_left (Nt.succ n)
+                            (Nt.add (Nt.mul (Nt.succ n) m) m)
+
+                _   =nt (Nt.add (Nt.succ n)
+                        (Nt.succ (Nt.add (Nt.mul (Nt.succ n) m) m)))
+                        := Nt.eq_symm (Nt.add_succ_right (Nt.succ n)
+                                (Nt.add (Nt.mul (Nt.succ n) m) m))
+
+                _   =nt (Nt.add (Nt.succ n)
+                        (Nt.add (Nt.mul (Nt.succ n) m) (Nt.succ m)))
+                        := Nt.add_congr_right (Nt.eq_symm (
+                            Nt.add_succ_right (Nt.mul (Nt.succ n) m) m))
+
+                _   =nt (Nt.add (Nt.add (Nt.succ n)
+                            (Nt.mul (Nt.succ n) m)) (Nt.succ m))
+                        := Nt.add_ass (Nt.succ n)
+                                (Nt.mul (Nt.succ n) m) (Nt.succ m)
+
+                _   =nt (Nt.add (Nt.mul (Nt.succ n) (Nt.succ m))
+                            (Nt.succ m))
+                        := Nt.add_congr_left (Nt.eq_symm
+                            (Nt.mul_succ_right (Nt.succ n) m))
+
+
+        intro m
+        apply Nt.induction P_step h_step_base h_step_step m
+
+    let P_b (a : Nt) : Prop := P a b
+
+    apply Nt.induction P_b (h_base b) (h_step b) a
+
+
+theorem Nt.mul_comm (a b : Nt) : Nt.mul a b =nt Nt.mul b a := by
+
+    let P (n m : Nt) : Prop := Nt.mul n m =nt Nt.mul m n
+
+    have h_base : ∀ (m : Nt), P Nt.zero m := by
+
+        let P_base (m : Nt) : Prop := P Nt.zero m
+
+        have h_base_base : P Nt.zero Nt.zero := by
+
+            apply Nt.eq_rfl
+
+        have h_base_step :
+            ∀ (m : Nt), P Nt.zero m → P Nt.zero (Nt.succ m) := by
+
+            intro m hPm
+
+            calc
+                (Nt.mul Nt.zero (Nt.succ m))
+                    =nt Nt.zero
+                        := Nt.mul_zero_left (Nt.succ m)
+
+                _   =nt Nt.mul (Nt.succ m) Nt.zero
+                        := Nt.eq_symm (Nt.mul_zero_right (Nt.succ m))
+
+        intro m
+        apply Nt.induction P_base h_base_base h_base_step m
+
+    have h_step : ∀ (m : Nt), ∀ (n : Nt),
+        P n m → P (Nt.succ n) m := by
+
+        let P_step (m : Nt) : Prop :=
+            ∀ (n : Nt), P n m → P (Nt.succ n) m
+
+        have h_step_base :
+            ∀ (n : Nt), P n Nt.zero → P (Nt.succ n) Nt.zero := by
+
+            intro n hPn
+
+            calc
+                (Nt.mul (Nt.succ n) Nt.zero)
+                    =nt Nt.zero
+                        := Nt.mul_zero_right (Nt.succ n)
+
+                _   =nt (Nt.mul Nt.zero (Nt.succ n))
+                        := Nt.eq_symm (Nt.mul_zero_left (Nt.succ n))
+
+        have h_step_step :
+            ∀ (m : Nt),
+                (∀ (n : Nt), P n m → P (Nt.succ n) m)
+                →
+                (∀ (n : Nt),  P n (Nt.succ m) →
+                    P (Nt.succ n) (Nt.succ m))
+            := by
+
+            intro m h_step_n n hPnsuccm
+
+            calc
+                (Nt.mul (Nt.succ n) (Nt.succ m))
+                    =nt Nt.add (Nt.mul n (Nt.succ m)) (Nt.succ m)
+                        := Nt.mul_succ_left n (Nt.succ m)
+
+                _   =nt Nt.add (Nt.succ m) (Nt.mul n (Nt.succ m))
+                        := Nt.add_comm
+                            (Nt.mul n (Nt.succ m)) (Nt.succ m)
+
+                _   =nt Nt.add (Nt.succ m) (Nt.mul (Nt.succ m) n)
+                        := Nt.add_congr_right hPnsuccm
+
+                _   =nt Nt.mul (Nt.succ m) (Nt.succ n)
+                        := Nt.eq_symm (Nt.mul_succ_right (Nt.succ m) n)
+
+        intro m
+        apply Nt.induction P_step h_step_base h_step_step m
+
+    let P_b (a : Nt) : Prop := P a b
+
+    apply Nt.induction P_b (h_base b) (h_step b) a
+
+
+theorem Nt.mul_congr_right {a b c : Nt} (h : b =nt c) :
+    Nt.mul a b =nt Nt.mul a c := by
+
+    let P (n : Nt) : Prop :=
+        (b =nt c) → (Nt.mul n b =nt Nt.mul n c)
+
+    have h_base : P Nt.zero := by
+
+        intro hbeqc
+
+        calc
+            (Nt.mul Nt.zero b)
+                =nt Nt.zero
+                    := Nt.mul_zero_left b
+
+            _   =nt (Nt.mul Nt.zero c)
+                    := Nt.eq_symm (Nt.mul_zero_left c)
+
+    have h_step : ∀ (n : Nt), P n → P (Nt.succ n) := by
+
+        intro n hPn hbeqc
+
+        calc
+            (Nt.mul (Nt.succ n) b)
+                =nt (Nt.add (Nt.mul n b) b)
+                    := Nt.mul_succ_left n b
+
+            _   =nt (Nt.add (Nt.mul n c) b)
+                    := Nt.add_congr_left (hPn hbeqc)
+
+            _   =nt (Nt.add (Nt.mul n c) c)
+                    := Nt.add_congr_right hbeqc
+
+            _   =nt (Nt.mul (Nt.succ n) c)
+                    := Nt.eq_symm (Nt.mul_succ_left n c)
+
+    let P_a := Nt.induction P h_base h_step a
+    apply P_a h
+
+
+theorem Nt.mul_congr_left {a b c : Nt} (h : b =nt c) :
+    Nt.mul b a =nt Nt.mul c a := by
+
+    calc
+        (Nt.mul b a)
+            =nt (Nt.mul a b)
+                := Nt.mul_comm b a
+
+        _   =nt (Nt.mul a c)
+                := Nt.mul_congr_right h
+
+        _   =nt (Nt.mul c a)
+                := Nt.mul_comm a c
+
+
+theorem mul_zero_iff_factors_zero {a b : Nt} :
+    (Nt.mul a b =nt Nt.zero) ↔ (a =nt Nt.zero) ∨ (b =nt Nt.zero) := by
+
+    constructor
+    · intro habeqzero
+
+      by_cases haeqzero : a =nt Nt.zero
+      · left
+        exact haeqzero
+
+      · by_cases hbeqzero : b =nt Nt.zero
+        · right
+          exact hbeqzero
+
+        · have ⟨c, haeqsuccc, huniquec⟩ := Nt.unique_ante haeqzero
+          have ⟨d, hbeqsuccd, huniqued⟩ := Nt.unique_ante hbeqzero
+
+          have hsucczero :
+            Nt.succ (Nt.add c (Nt.mul (Nt.succ c) d)) =nt Nt.zero := by
+
+            calc
+                (Nt.succ (Nt.add c (Nt.mul (Nt.succ c) d)))
+                    =nt (Nt.add (Nt.succ c) (Nt.mul (Nt.succ c) d))
+                        := Nt.eq_symm (Nt.add_succ_left c
+                            (Nt.mul (Nt.succ c) d))
+
+                _   =nt (Nt.mul (Nt.succ c) (Nt.succ d))
+                        := Nt.eq_symm (Nt.mul_succ_right (Nt.succ c) d)
+
+                _   =nt (Nt.mul a (Nt.succ d))
+                        := Nt.mul_congr_left haeqsuccc
+
+                _   =nt (Nt.mul a b)
+                        := Nt.mul_congr_right hbeqsuccd
+
+                _   =nt Nt.zero
+                        := habeqzero
+
+          exfalso
+          apply Nt.succ_ne_zero
+            (Nt.add c (Nt.mul (Nt.succ c) d)) hsucczero
+
+
+    · intro habzero
+      rcases habzero with haeqzero | hbeqzero
+
+      · calc
+            (Nt.mul a b)
+                =nt (Nt.mul Nt.zero b)
+                    := Nt.mul_congr_left haeqzero
+
+            _   =nt Nt.zero
+                    := Nt.mul_zero_left b
+
+      · calc
+            (Nt.mul a b)
+                =nt (Nt.mul a Nt.zero)
+                    := Nt.mul_congr_right hbeqzero
+
+            _   =nt Nt.zero
+                    := Nt.mul_zero_right a
+
+theorem Nt.mul_not_zero_if_factors_not_zero (a b : Nt)
+    (hanezero : (a =nt Nt.zero) → False)
+    (hbnezero : (b =nt Nt.zero) → False) :
+
+    ((Nt.mul a b =nt Nt.zero) → False) := by
+
+    intro habeqzero
+
+    have haeqzeroANDbeqzero := mul_zero_iff_factors_zero.mp habeqzero
+
+    rcases haeqzeroANDbeqzero with haeqzero | hbeqzero
+    · apply hanezero
+      exact haeqzero
+    · apply hbnezero
+      exact hbeqzero
+
+
+theorem Nt.mul_distr_right (a b c : Nt) :
+    Nt.mul a (Nt.add b c) =nt Nt.add (Nt.mul a b) (Nt.mul a c) := by
+
+    let P (n : Nt) : Prop := Nt.mul n (Nt.add b c) =nt
+        Nt.add (Nt.mul n b) (Nt.mul n c)
+
+    have h_base : P Nt.zero := by
+
+        calc
+            (Nt.mul Nt.zero (Nt.add b c))
+                =nt Nt.zero
+                    := Nt.mul_zero_left (Nt.add b c)
+
+            _   =nt Nt.add Nt.zero Nt.zero
+                    := Nt.eq_symm (Nt.add_zero_right Nt.zero)
+
+            _   =nt Nt.add (Nt.mul Nt.zero b) Nt.zero
+                    := Nt.add_congr_left (
+                        Nt.eq_symm (Nt.mul_zero_left b))
+
+            _   =nt Nt.add (Nt.mul Nt.zero b) (Nt.mul Nt.zero c)
+                    := Nt.add_congr_right (
+                        Nt.eq_symm (Nt.mul_zero_left c))
+
+    have h_step : ∀ (n : Nt), P n → P (Nt.succ n) := by
+
+        intro n hPn
+
+        calc
+            (Nt.mul (Nt.succ n) (Nt.add b c))
+                =nt (Nt.add (Nt.mul n (Nt.add b c)) (Nt.add b c))
+                    := Nt.mul_succ_left n (Nt.add b c)
+
+            _   =nt (Nt.add (Nt.add (Nt.mul n b) (Nt.mul n c))
+                        (Nt.add b c))
+                    := Nt.add_congr_left hPn
+
+            _   =nt (Nt.add (Nt.mul n b)
+                        (Nt.add (Nt.mul n c) (Nt.add b c)))
+                    := Nt.eq_symm (Nt.add_ass 
+                        (Nt.mul n b) (Nt.mul n c) (Nt.add b c))
+
+            _   =nt (Nt.add (Nt.mul n b)
+                        (Nt.add (Nt.mul n c) (Nt.add c b)))
+                    := Nt.add_congr_right (Nt.add_congr_right (
+                        Nt.add_comm b c))
+
+            _   =nt (Nt.add (Nt.mul n b)
+                        (Nt.add (Nt.add (Nt.mul n c) c) b))
+                    := Nt.add_congr_right (Nt.add_ass (Nt.mul n c) c b)
+
+            _   =nt (Nt.add (Nt.mul n b)
+                        (Nt.add (Nt.mul (Nt.succ n) c) b))
+                    := Nt.add_congr_right (Nt.add_congr_left (
+                        Nt.eq_symm (Nt.mul_succ_left n c)))
+
+            _   =nt (Nt.add (Nt.mul n b)
+                        (Nt.add b (Nt.mul (Nt.succ n) c)))
+                    := Nt.add_congr_right (
+                        Nt.add_comm (Nt.mul (Nt.succ n) c) b)
+
+            _   =nt (Nt.add (Nt.add (Nt.mul n b) b)
+                        (Nt.mul (Nt.succ n) c))
+                    := Nt.add_ass (Nt.mul n b) b (Nt.mul (Nt.succ n) c)
+
+            _   =nt (Nt.add (Nt.mul (Nt.succ n) b)
+                        (Nt.mul (Nt.succ n) c))
+                    := Nt.add_congr_left (Nt.eq_symm (
+                        Nt.mul_succ_left n b))
+
+    apply Nt.induction P h_base h_step a
+
+
+theorem Nt.mul_distr_left (a b c : Nt) :
+    Nt.mul (Nt.add b c) a =nt Nt.add (Nt.mul b a) (Nt.mul c a) := by
+
+    calc
+        (Nt.mul (Nt.add b c) a)
+            =nt Nt.mul a (Nt.add b c)
+                := Nt.mul_comm (Nt.add b c) a
+
+        _   =nt Nt.add (Nt.mul a b) (Nt.mul a c)
+                := Nt.mul_distr_right a b c
+
+        _   =nt Nt.add (Nt.mul b a) (Nt.mul a c)
+                := Nt.add_congr_left (Nt.mul_comm a b)
+
+        _   =nt Nt.add (Nt.mul b a) (Nt.mul c a)
+                := Nt.add_congr_right (Nt.mul_comm a c)
+
+
+theorem Nt.mul_ass (a b c : Nt) :
+    Nt.mul (Nt.mul a b) c =nt Nt.mul a (Nt.mul b c) := by
+
+    let P (n : Nt) : Prop :=
+        Nt.mul (Nt.mul a b) n =nt Nt.mul a (Nt.mul b n)
+
+    have h_base : P Nt.zero := by
+
+        calc
+            (Nt.mul (Nt.mul a b) Nt.zero)
+                =nt Nt.zero
+                    := Nt.mul_zero_right (Nt.mul a b)
+
+            _   =nt Nt.mul a Nt.zero
+                    := Nt.eq_symm (Nt.mul_zero_right a)
+
+            _   =nt Nt.mul a (Nt.mul b Nt.zero)
+                    := Nt.mul_congr_right (Nt.eq_symm (
+                        Nt.mul_zero_right b))
+
+    have h_step : ∀ (n : Nt), P n → P (Nt.succ n) := by
+        intro n hPn
+
+        calc
+            (Nt.mul (Nt.mul a b) (Nt.succ n))
+                =nt (Nt.add (Nt.mul a b) (Nt.mul (Nt.mul a b) n))
+                    := Nt.mul_succ_right (Nt.mul a b) n
+
+            _   =nt (Nt.add (Nt.mul a b) (Nt.mul a (Nt.mul b n) ))
+                    := Nt.add_congr_right hPn
+
+            _   =nt (Nt.mul a (Nt.add b (Nt.mul b n)))
+                    := Nt.eq_symm (Nt.mul_distr_right a b (Nt.mul b n))
+
+            _   =nt (Nt.mul a (Nt.mul b (Nt.succ n)))
+                    := Nt.mul_congr_right (Nt.eq_symm (
+                        Nt.mul_succ_right b n))
+
+    apply Nt.induction P h_base h_step c
+
+
+theorem Nt.gt_mul_const (a b c : Nt)
+    (hcpos : Nt.pos c) (hbgta : Nt.gt b a) :
+    Nt.gt (Nt.mul b c) (Nt.mul a c) := by
+
+    rcases (Nt.gt_exists_pos b a).mp hbgta with ⟨d, hdpos, hbeqad⟩
+
+    apply (Nt.gt_exists_pos (Nt.mul b c) (Nt.mul a c)).mpr
+
+    exists (Nt.mul d c)
+
+    constructor
+    · apply Nt.mul_not_zero_if_factors_not_zero d c hdpos hcpos
+    · calc
+        (Nt.mul b c)
+            =nt Nt.mul (Nt.add a d) c
+                := Nt.mul_congr_left hbeqad
+
+        _   =nt Nt.add (Nt.mul a c) (Nt.mul d c)
+                := Nt.mul_distr_left c a d
+
+
+theorem Nt.mul_canc_right {a b c : Nt}
+    (hcpos : Nt.pos c) (haceqbc : (Nt.mul a c) =nt (Nt.mul b c)) :
+    a =nt b := by
+
+    have h_contradiction (x y : Nt)
+        (hxceqyc : Nt.mul x c =nt Nt.mul y c)
+        (hxgty : Nt.gt x y) : False := by
+
+        have hxcgtyc : Nt.gt (Nt.mul x c) (Nt.mul y c) :=
+            Nt.gt_mul_const y x c hcpos hxgty
+
+        rcases hxcgtyc with ⟨hxcgeyc, hxcneyc⟩
+
+        apply hxcneyc
+        exact hxceqyc
+
+    rcases (Nt.order_trichotomy a b) with haeqb | hagtb | hbgta
+    · exact haeqb
+
+    · exfalso
+      apply (h_contradiction a b haceqbc hagtb)
+
+    · exfalso
+      have hbceqac := Nt.eq_symm haceqbc
+      apply (h_contradiction b a hbceqac hbgta)
+
+
+/- Multiplication theorems -/
+
+
+noncomputable def Nt.one : Nt := (Nt.succ Nt.zero)
+noncomputable def Nt.two : Nt := (Nt.succ Nt.one)
+
+theorem Nt.mul_one_right (a : Nt) : (Nt.mul a Nt.one) =nt a := by
+    unfold Nt.one
+
+    calc
+        (Nt.mul a (Nt.succ Nt.zero))
+            =nt (Nt.add a (Nt.mul a Nt.zero))
+                := Nt.mul_succ_right a Nt.zero
+
+        _   =nt (Nt.add a Nt.zero)
+                := Nt.add_congr_right (Nt.mul_zero_right a)
+
+        _   =nt a
+                := Nt.add_zero_right a
+
+theorem Nt.mul_one_left (a : Nt) : (Nt.mul Nt.one a) =nt a := by
+    calc
+        (Nt.mul Nt.one a)
+            =nt (Nt.mul a Nt.one)
+                := Nt.mul_comm Nt.one a
+
+        _   =nt a
+                := Nt.mul_one_right a
+
+theorem Nt.mul_two_right (a : Nt) :
+    (Nt.mul a Nt.two) =nt (Nt.add a a) := by
+
+    unfold Nt.two
+
+    calc
+        (Nt.mul a (Nt.succ Nt.one))
+            =nt Nt.add a (Nt.mul a Nt.one)
+                := Nt.mul_succ_right a Nt.one
+
+        _   =nt Nt.add a a
+                := Nt.add_congr_right (Nt.mul_one_right a)
+
+
+theorem Nt.mul_two_left (a : Nt) :
+    (Nt.mul Nt.two a) =nt (Nt.add a a) := by
+
+    calc
+        (Nt.mul Nt.two a)
+            =nt (Nt.mul a Nt.two)
+                := Nt.mul_comm Nt.two a
+
+        _   =nt (Nt.add a a)
+                := Nt.mul_two_right a
+
+
+theorem euclidean_algorithm (n q : Nt) (hqpos : Nt.pos q) :
+    ∃ m r : Nt, (n =nt Nt.add (Nt.mul m q) r) ∧ (Nt.gt q r) := by
+
+    let P (a : Nt) : Prop :=
+        ∃ m r : Nt, (a =nt Nt.add (Nt.mul m q) r) ∧ (Nt.gt q r)
+
+    have h_base : P Nt.zero := by
+        exists Nt.zero, Nt.zero
+
+        constructor
+        · calc
+            Nt.zero
+                =nt Nt.add Nt.zero Nt.zero
+                    := Nt.eq_symm (Nt.add_zero_right Nt.zero)
+
+            _   =nt Nt.add (Nt.mul Nt.zero q) Nt.zero
+                    := Nt.add_congr_left (Nt.eq_symm (
+                        Nt.mul_zero_left q))
+        · constructor
+          · exists q
+            apply (Nt.eq_symm (Nt.add_zero_left q))
+          · exact hqpos
+
+    have h_step : ∀ a : Nt, P a → P (Nt.succ a) := by
+
+        intro a hPa
+
+        rcases hPa with ⟨m, r, hconj⟩
+        rcases hconj with ⟨haeqmqr, hqgtr⟩
+
+        by_cases hqeqsuccr : q =nt (Nt.succ r)
+        · exists (Nt.succ m), Nt.zero
+
+          constructor
+          · have hsuccaeqsuccmqr := Nt.succ_congr haeqmqr
+
+            calc
+                (Nt.succ a)
+                    =nt Nt.succ (Nt.add (Nt.mul m q) r)
+                        := hsuccaeqsuccmqr
+
+                _   =nt Nt.add (Nt.mul m q) (Nt.succ r)
+                        := Nt.eq_symm (Nt.add_succ_right (Nt.mul m q) r)
+
+                _   =nt Nt.add (Nt.mul m q) q
+                        := Nt.add_congr_right (Nt.eq_symm hqeqsuccr)
+
+                _   =nt Nt.mul (Nt.succ m) q
+                        := Nt.eq_symm (Nt.mul_succ_left m q)
+
+                _   =nt Nt.add (Nt.mul (Nt.succ m) q) Nt.zero
+                        := Nt.eq_symm (
+                            Nt.add_zero_right (Nt.mul (Nt.succ m) q))
+
+          · constructor
+
+            · exists q
+              apply Nt.eq_symm (Nt.add_zero_left q)
+
+            · exact hqpos
+
+        · have hqgesuccr := (Nt.gt_iff_ge_succ q r).mp hqgtr
+
+          exists m, (Nt.succ r)
+
+          constructor
+          · calc
+                (Nt.succ a)
+                    =nt (Nt.succ (Nt.add (Nt.mul m q) r))
+                        := Nt.succ_congr haeqmqr
+
+                _   =nt (Nt.add (Nt.mul m q) (Nt.succ r))
+                        := Nt.eq_symm (
+                            Nt.add_succ_right (Nt.mul m q) r)
+
+          · constructor
+            · exact hqgesuccr
+            · exact hqeqsuccr
+
+
+    apply Nt.induction P h_base h_step n
+
+
+/- Exponentiation definition -/
+
+
+axiom Nt.pow : Nt → Nt → Nt
+
+axiom Nt.pow_zero (a : Nt) :
+    Nt.pow a Nt.zero =nt Nt.one
+
+axiom Nt.pow_succ (a b : Nt) :
+    Nt.pow a (Nt.succ b) =nt Nt.mul a (Nt.pow a b)
+
+
+/- Exponentiation properties -/
+
+
+
+theorem Nt.pow_one (a : Nt) : Nt.pow a Nt.one =nt a := by
+    unfold Nt.one
+
+    calc
+        Nt.pow a (Nt.succ Nt.zero)
+            =nt Nt.mul a (Nt.pow a Nt.zero)
+                := Nt.pow_succ a Nt.zero
+
+        _   =nt Nt.mul a Nt.one
+                := Nt.mul_congr_right (Nt.pow_zero a)
+
+        _   =nt a
+                := Nt.mul_one_right a
+
+
+theorem Nt.pow_two (a : Nt) : Nt.pow a Nt.two =nt Nt.mul a a := by
+    unfold Nt.two
+
+    calc
+        Nt.pow a (Nt.succ Nt.one)
+            =nt Nt.mul a (Nt.pow a Nt.one)
+                := Nt.pow_succ a Nt.one
+
+        _   =nt Nt.mul a a
+                := Nt.mul_congr_right (Nt.pow_one a)
+
+
+theorem Nt.quadratic_identity (a b : Nt) :
+    Nt.pow (Nt.add a b) Nt.two =nt
+
+    Nt.add (Nt.pow a Nt.two)
+        (Nt.add
+            (Nt.mul Nt.two (Nt.mul a b))
+            (Nt.pow b Nt.two))
+
+    := by
+
+    calc
+        (Nt.pow (Nt.add a b) Nt.two)
+            =nt (Nt.mul (Nt.add a b) (Nt.add a b))
+                := Nt.pow_two (Nt.add a b)
+
+        _   =nt (Nt.add (Nt.mul (Nt.add a b) a) (Nt.mul (Nt.add a b) b))
+                := Nt.mul_distr_right (Nt.add a b) a b
+
+        _   =nt (Nt.add
+                    (Nt.add (Nt.mul a a) (Nt.mul b a))
+                    (Nt.mul (Nt.add a b) b))
+                := Nt.add_congr_left (Nt.mul_distr_left a a b)
+
+        _   =nt (Nt.add
+                    (Nt.add (Nt.mul a a) (Nt.mul b a))
+                    (Nt.add (Nt.mul a b) (Nt.mul b b)))
+                := Nt.add_congr_right (Nt.mul_distr_left b a b)
+
+        _   =nt (Nt.add
+                    (Nt.add (Nt.mul a a) (Nt.mul a b))
+                    (Nt.add (Nt.mul a b) (Nt.mul b b)))
+                := Nt.add_congr_left (Nt.add_congr_right (
+                    Nt.mul_comm b a))
+
+        _   =nt (Nt.add
+                    (Nt.add
+                        (Nt.add (Nt.mul a a) (Nt.mul a b))
+                        (Nt.mul a b))
+                    (Nt.mul b b))
+                := Nt.add_ass (Nt.add (Nt.mul a a) (Nt.mul a b))
+                    (Nt.mul a b) (Nt.mul b b)
+
+        _   =nt (Nt.add
+                    (Nt.add
+                        (Nt.mul a a)
+                        (Nt.add (Nt.mul a b) (Nt.mul a b)))
+                    (Nt.mul b b))
+                := Nt.add_congr_left (Nt.eq_symm (
+                    Nt.add_ass (Nt.mul a a) (Nt.mul a b) (Nt.mul a b)))
+
+        _   =nt (Nt.add
+                    (Nt.add
+                        (Nt.mul a a)
+                        (Nt.mul Nt.two (Nt.mul a b)))
+                    (Nt.mul b b))
+                := Nt.add_congr_left (Nt.add_congr_right (
+                    Nt.eq_symm (Nt.mul_two_left (Nt.mul a b))))
+
+        _   =nt (Nt.add
+                    (Nt.mul a a)
+                    (Nt.add
+                        (Nt.mul Nt.two (Nt.mul a b))
+                        (Nt.mul b b)))
+                := Nt.eq_symm (Nt.add_ass (Nt.mul a a)
+                    (Nt.mul Nt.two (Nt.mul a b)) (Nt.mul b b))
+
+        _   =nt (Nt.add
+                    (Nt.pow a Nt.two)
+                    (Nt.add
+                        (Nt.mul Nt.two (Nt.mul a b))
+                        (Nt.mul b b)))
+                := Nt.add_congr_left (Nt.eq_symm (Nt.pow_two a))
+
+        _   =nt (Nt.add
+                    (Nt.pow a Nt.two)
+                    (Nt.add
+                        (Nt.mul Nt.two (Nt.mul a b))
+                        (Nt.pow b Nt.two)))
+                := Nt.add_congr_right (Nt.add_congr_right (
+                    Nt.eq_symm (Nt.pow_two b)))
+
+
