St/Rel.lean
@@ -1,0 +1,60 @@
+axiom Rel : St → St → Type
+
+axiom Func.uniq {A B : St} (f : Func A B) :
+
+    ∀ x y1 y2 : St, St.mem x A →
+        Func.app f x y1 → Func.app f x y2 → (y1 =st y2)
+
+axiom Func.from_Rel {A B : St} {P : St → St → Prop}
+  (h_tot : ∀ x : St, St.mem x A → ∃ y, St.mem y B ∧ P x y)
+  (h_uniq : ∀ x y1 y2 : St, St.mem x A → P x y1 → P x y2 → (y1 =st y2))
+  : Func A B
+
+
+axiom Func.satisfy_Rel {A B : St} {P : St → St → Prop}
+  (h_tot : ∀ x : St, St.mem x A → ∃ y, St.mem y B ∧ P x y)
+  (h_uniq : ∀ x y1 y2 : St, St.mem x A → P x y1 → P x y2 → (y1 =st y2))
+  (x : St) (hx : St.mem x A) :
+
+  P x (Func.app (Func.from_Rel h_tot h_uniq) x)
+
+noncomputable def Func.comp {A B C : St} (g : Func B C) (f : Func A B) :
+  Func A C :=
+
+  let P_comp (x z : St) : Prop :=
+    z =st (Func.app g (Func.app f x))
+
+  have h_tot : ∀ x : St, St.mem x A →
+    ∃ z : St, St.mem z C ∧ P_comp x z := by
+
+    intro x hxmemA
+    have ⟨y, hymemB, hyeqfx⟩ := Func.tot f x hxmemA
+    have ⟨z, hzmemC, hzeqgy⟩ := Func.tot g y hymemB
+
+    exists z
+    constructor
+    . exact hzmemC
+    . calc
+        z =st Func.app g y
+            := hzeqgy
+
+        _ =st Func.app g (Func.app f x)
+            := Func.app_congr_right hyeqfx
+
+  have h_uniq : ∀ x z1 z2, St.mem x A → P_comp x z1 → P_comp x z2 →
+      (z1 =st z2) := by
+
+    intro x z1 z2 hxmemA hz1eqgfx hz2eqgfx
+
+    have ⟨y, hymemB, hyeqfx⟩ := Func.tot f x hxmemA
+    have ⟨z, hzmemC, hzeqgy⟩ := Func.tot g y hymemB
+
+    calc
+        z1  =st Func.app g (Func.app f x)
+            := hz1eqgfx
+
+        _   =st z2
+            := St.eq_symm hz2eqgfx
+
+  Func.from_Rel h_tot h_uniq
+
