St/Russell.lean
@@ -1,57 +1,59 @@
 import St.Subset
 -- import Nt.Addition
 
-axiom set_exists_universal_specification (P : St → Prop) :
+axiom St.set_exists_universal_specification (P : St → Prop) :
     ∃ S : St,
-        ∀ y : St, mem y S ↔ P y
+        ∀ y : St, St.mem y S ↔ P y
 
-theorem russell_set_exists_replacement (A : St) (P : St → St → Prop) :
+theorem St.russell_set_exists_replacement (A : St)
+    (P : St → St → Prop) :
+
     ∃ S : St,
-        ∀ y : St, mem y S ↔ (∃ x : St, mem x A ∧ (P x y)) := by
+        ∀ y : St, St.mem y S ↔ (∃ x : St, St.mem x A ∧ (P x y)) := by
 
-    let PU (y : St) : Prop := (∃ x : St, mem x A ∧ (P x y))
+    let PU (y : St) : Prop := (∃ x : St, St.mem x A ∧ (P x y))
 
     apply set_exists_universal_specification PU
 
-theorem russell_set_exists_specification (A : St) (P : St → Prop) :
+theorem St.russell_set_exists_specification (A : St) (P : St → Prop) :
     ∃ S : St,
-        ∀ y : St, mem y S ↔ (mem y A ∧ (P y)) := by
+        ∀ y : St, St.mem y S ↔ (St.mem y A ∧ (P y)) := by
 
-    let PU (y : St) : Prop := mem y A ∧ (P y)
+    let PU (y : St) : Prop := St.mem y A ∧ (P y)
 
     apply set_exists_universal_specification PU
 
-theorem russell_set_exists_general_uni (A : St) :
+theorem St.russell_set_exists_general_uni (A : St) :
     ∃ S : St,
-        ∀ y : St, mem y S ↔ ∃ x : St, mem x A ∧ mem y x := by
+        ∀ y : St, St.mem y S ↔ ∃ x : St, St.mem x A ∧ St.mem y x := by
 
-    let PU (y : St) : Prop := ∃ x : St, mem x A ∧ mem y x
+    let PU (y : St) : Prop := ∃ x : St, St.mem x A ∧ St.mem y x
 
-    apply set_exists_universal_specification PU
+    apply St.set_exists_universal_specification PU
 
-theorem russell_set_exists_pair (a b : St) :
+theorem St.russell_set_exists_pair (a b : St) :
     ∃ S : St,
-        ∀ y : St, mem y S ↔ ((y =st a) ∨ (y =st b)) := by
+        ∀ y : St, St.mem y S ↔ ((y =st a) ∨ (y =st b)) := by
 
     let PU (y : St) : Prop := ((y =st a) ∨ (y =st b))
 
-    apply set_exists_universal_specification PU
+    apply St.set_exists_universal_specification PU
 
-theorem russell_set_exists_singlet (a : St) :
+theorem St.russell_set_exists_singlet (a : St) :
     ∃ S : St,
-        ∀ y : St, mem y S ↔ (y =st a) := by
+        ∀ y : St, St.mem y S ↔ (y =st a) := by
 
     let PU (y : St) : Prop := (y =st a)
 
-    apply set_exists_universal_specification PU
+    apply St.set_exists_universal_specification PU
 
-theorem russell_set_exists_empty :
+theorem St.russell_set_exists_empty :
     ∃ S : St,
-        ∀ y : St, mem y S ↔ False := by
+        ∀ y : St, St.mem y S ↔ False := by
 
     let PU (y : St) : Prop := False
 
-    apply set_exists_universal_specification PU
+    apply St.set_exists_universal_specification PU
 
 
 /-
@@ -61,8 +63,8 @@ axiom set_succ (x : St) : (succ x) =st (uni x (singlet x))
 
 theorem russell_set_infinity :
     ∃ S : St,
-        mem empty S ∧
-        ∀ y : St, mem y S ↔ mem (succ y) S := by
+        St.mem empty S ∧
+        ∀ y : St, St.mem y S ↔ St.mem (succ y) S := by
 
     let PU (y : St) : Prop :=
             (y empty) ∧ ∃ n : St, n =st (succ y)
